#### Light clock and invariant interval: 

$$
\begin{gather}
\Delta s^{2} = \Delta t^{2}-\Delta x^{2}
\end{gather}
$$
Where the spacetime interval $\Delta s$ is invariant. It doesn't change depending on reference frame. 

#### Lorentz Tranformations

1D motion $\beta$ in $+x$ direction:
- $t=\gamma(t'+\beta x)$
- $x=\gamma(\beta t+x')$
You can use the equations to compare the coordinate systems. 
- $t' = \gamma(t-\beta x)$
- $x' = \gamma(-\beta t +x)$

The transformation as a matrix: q
$$
\begin{gather}
\begin{pmatrix}
x' \\
t' \\

\end{pmatrix} = 
\begin{pmatrix}
\gamma & -\gamma_{\beta} \\
-\gamma_{\beta} & \gamma
\end{pmatrix}
\begin{pmatrix}
x \\
t
\end{pmatrix}=\gamma
\begin{pmatrix}
1 & \beta \\
-\beta &1
\end{pmatrix}
\begin{pmatrix}
x \\
t
\end{pmatrix}
\end{gather}
$$
Thus if $x=\beta t$ in the lab frame, then $t' = \gamma(t-\beta(\beta t))=\gamma t(1-\beta^{2})=\frac{t}{\gamma}$ or time dialation. 

Back to E&M!

Section 5.6 in Purcell: 

If $V=0$ then the electric field is $E=\frac{kQ}{r^{2}}$ with spherically symmetric arrows. 
![[Pasted image 20240227123247.png|center]]

We have that $E_{x} = Qk \frac{1}{r^{2}}\cos\theta = \frac{Qxk}{(x^{2}+z^{2})^{3/2}}$, $E_{z} = kQ \frac{1}{r^{2}}\sin\theta \frac{Qzk}{(x^{2}+z^{2})^{3/2}}$ 

The form of the Lorentz equations is: 
$$
\begin{gather}
x = \gamma(x'-\beta ct)\\ \\
t = \gamma\left( t'-\frac{\beta x'}{c} \right) \\ \\ 
y=y' \hspace{.5cm}z=z' \\ \\

\text{parallel:} \hspace{.2cm}E'_{x} = E_{x} =. \frac{Qk(\gamma x')}{[(\gamma x')^{2}+z'^{2}]^{3/2}} \\ \\ 

\text{perp} \hspace{.2cm} E'_{z} = \gamma E_{z} = \frac{\gamma k(Qz')}{[(\gamma x')^{2}+z'^{2}]^{3/2}}
\end{gather}
$$
where we have assumed that $t'=t=0$. THe field lines ties into the charge:
$$
\begin{gather}
\frac{E'_{z}}{E'_{x}} = \frac{z'}{x'}
\end{gather}
$$
More algebra! We want to know the magnitude of the E in the other frame: 
$$
\begin{gather}
E'^{2} = (E'_{x} )^{2}+(E'_{z})^{2} = \frac{k^{2}\gamma^{2}Q^{2}(x'^{2}+z'^{2})}{\underbrace{ [(\gamma x')^{2}+z'^{2}]^{3} }_{ \text{factor} \hspace{.2cm} \gamma^6 }} \\ \\ 
\text{where:} \hspace{.2cm}\gamma^{2} = \frac{1}{1-\beta^{2}} \\ \\ 
\frac{k^{2}\gamma^{2}Q^{2}(x'^{2}+z'^{2})}{ [\gamma^6(x')^{2}+(1-\beta^{2})z'^{2}]^{3} } \\ \\ 
 \frac{k^{2}\gamma^{2}Q^{2}(x'^{2}+z'^{2})}{ [\gamma^6(x')^{2}+(1-\beta^{2})z'^{2}]^{3} } \cdot \frac{\frac{1}{(x'^{2}+z'^{2})^{3}}}{\frac{1}{(x'^{2}+z'^{2})^{3}}} \\ \\ 
  = \frac{k^{2}Q^{2}(1-\beta^{2})^{2}}{(x'^{2}+z'^{2})^{2}} \cdot \frac{1}{ 1- \left( \frac{\beta^{2}z'^{2}}{(x'^{2}+z'^{2})} \right)^{3}} = \\ \\ 
E' = \frac{Qk}{r^{2}} \frac{1-\beta^{2}}{(1-\beta^{2}\sin ^{2}\theta')^{3/2}} \\ \\ 
\text{when} \hspace{.2cm} \theta' = \frac{\pi}{2} \hspace{.5cm} E'_{\perp} = \frac{\gamma kQ}{r'^{2}} \\ \\ 
\theta' = 0 \hspace{.5cm}E'_{\parallel} = \frac{1}{\gamma^{2}}

\end{gather}
$$Equation break time!

![[Pasted image 20240227123822.png|center|300]]

