Situation 1
$I = \lambda v$
- the rate at which charges are going by
- no net $\lambda$
- $F = q(v\times B)$

![[Pasted image 20240229114906 1.png|center|300]]

Situation 2
From Gauss's law we have that 
$$
\begin{gather}
E'(2\pi r'l) = \frac{\lambda'}{2\pi e_{0}r'} \sim \frac{1}{r}
\end{gather}
$$
![[Pasted image 20240229115451 1.png|center|300]]

New situation 1; 
there are 3 $\beta$ and $\gamma$s: 
$$
\begin{gather}
\beta = \frac{v}{c} (Charge), \hspace{.5cm} \beta_{0} \frac{V_{0}}{c}(\text{electron fluid}) \\ \\ \hspace{.5cm}\beta_{0}' \rightarrow \text{electron beta in the q frame} \hspace{.2cm}
\end{gather}
$$

![[Pasted image 20240229120333 1.png|center|300]]
Where the above picture is the lab frame:

In the charge frame:
![[Pasted image 20240229121032 1.png|center|300]]

be wary of the Einstein velocity addition formula!

We have that:
$$
\begin{gather}
\beta_{0}' = \frac{\beta_{0} - \beta}{1-\beta\beta_{0}} \\ \\

\gamma_{0}' = \frac{1}{\sqrt{ 1-\beta_{0}'^{2} }} = \gamma\gamma_{0}(1-\beta\beta_{0}) \hspace{.5cm}\text{see the video} \hspace{.2cm} \\ \\
(1-\beta\beta_{0}) \leftarrow \text{transformation to charge frame} \hspace{.2cm}
\end{gather}
$$
Total linear charge density: 
$$
\begin{gather}
\lambda' = \underbrace{ \gamma\lambda_{0} }_{ ions } - \frac{\lambda_{1}}{\gamma_{0}} \hspace{.5cm} = \gamma\beta\beta_{0}\lambda_{0} \\ \\ 

\frac{\lambda_{1}}{\gamma_{0}} \leftarrow \text{negative charge density in electron frame} \hspace{.2cm} \\ \\

E_{r}' = \frac{\lambda'}{2\pi \epsilon_{0}r'} = \frac{\gamma\beta\beta_{0}\lambda_{0}}{2\pi\epsilon_{0}r'} \\ \\ 

F_{y}' = qE_{y}' = -\frac{1\gamma\beta\beta_{0}\lambda_{0}}{2\pi\epsilon_{0}r'} \leftarrow \text{force in the charge frame} \hspace{.2cm} \\ \\ 

\end{gather}
$$$$
\begin{gather}
I = v_{0}\lambda_{0} = \beta_{0}\lambda_{0} \\ \\ 
F_{y} = \frac{F_{y}'}{\gamma} = -\frac{q\beta\beta_{0}\lambda_{0}}{2\pi \epsilon_{0} } = -\frac{q\beta\beta_{0}\lambda_{0}c}{2\pi \epsilon_{0} c} = \frac{\left( \frac{V}{c}I \right)}{2\pi\epsilon_{0} rc}= -qv_{x}\left( \frac{I}{2\pi\epsilon_{0}rc^{2}} \right)
\end{gather} \\ \\
$$

![[Pasted image 20240229122223.png|center|300]]

If $\beta\ll 1$ then
$$
\begin{gather}
\gamma = (1-\beta^{2}) \approx 1+ \frac{1}{2}\beta^{2} \dots E = \lambda mc^{2} = \left( 1+ \frac{1}{2}\beta^{2} \right) mc^{2} = mc^{2} = 1+ \frac{1}{2}\beta^{2}mc^{2}
\text{where all the way to the right is rest energy!} \hspace{.2cm}
\end{gather}
$$