"Displacement" current: 
$$
\begin{gather}
\mu_{0}J \rightarrow \mu_{0}\left( J+ \epsilon_{0}  \frac{\partial E}{\partial t} \right) \\ \\
\nabla \cdot\left( \nabla \times B = \mu_{0}\left( J+\epsilon_{0} \frac{ \partial E }{ \partial t }  \right) \right) \\ \\ 
0 = \mu_{0}\nabla \cdot J +\mu_{0}\frac{ \partial \rho }{ \partial t }  \\ \\
= \mu_{0}(\nabla \cdot J+ \frac{ \partial \rho }{ \partial t } ) = 0
\end{gather}
$$
Theoretical Symmetry: 
From chapter six 
$$
\begin{gather}
\frac{E}{B}=c
\end{gather}
$$
