Traveling wave

![[Pasted image 20240416113839.png|center|300]]

We have the general wave equation 
$$
\begin{gather}
u_{tt} = \frac{1}{c^{2}}\triangle u 
\end{gather}
$$
where the solution is $E$. Thus the general solution of the wave equation is 
$$
\begin{gather}
E = E_{0}\cos(kx-\omega t)\hat{y} \hspace{.5cm} \frac{1}{l}=\frac{2\pi}{\lambda}=k \\ \\ 
B = B_{0}con(kx-\omega t) \hat{z}
\end{gather}
$$
We have that 
$$
\begin{gather}
\frac{E_{0}}{B_{0}} = c = \frac{\omega}{k}
\end{gather}
$$
Let's now analyze the same situation using the integral form of Faraday's law
$$
\begin{gather}
\underbrace{ \oint E\cdot dl }_{ hdE } = \underbrace{ \frac{ \partial \Phi_{B} }{ \partial t}  }_{ \frac{dB}{dt} hdx }\\ \\ 
\frac{dE_{y}}{dx} = \frac{dB}{dt}
\end{gather}
$$
![[Drawing 2024-04-16 11.28.12.excalidraw.svg|center|300]]

From Ampere's Law we have 
$$
\begin{gather}
\oint B \cdot dl =\frac{1}{c^{2}} \dot{\Phi}_{E} 
\end{gather}
$$
The picture is similar to the last one

![[Pasted image 20240416120304.png|center|300]]


Let's talk about Standing waves,

![[Pasted image 20240416120954.png|center|300]]

A little about cavities, 

![[Pasted image 20240416121332.png|center|300]]

Poynting's Theorem
$$
\begin{gather}
W_{EM} = W_{E} +W_{B} = \frac{1}{2}\int \left( \epsilon_{0}E^{2}+\frac{1}{\mu_{0}}B^{2} \right) \, d^{3}x
\end{gather}
$$
We want the work on $dq$ by $E,B$ during $dt$
![[Pasted image 20240416121947.png|center|300]]

$$
\begin{gather}
S = \frac{EB}{\mu_{0}} \\ \\ 
dW = F \cdot dl = dq(E+v\times B) \cdot \underbrace{ vdt }_{ dl } \leftarrow \hspace{.2cm} \text{ B fields do no work} \\ \\ 
\frac{dW}{dt} = E \cdot v\underbrace{ dq }_{ \rho d^{3}x } \hspace{.5cm}\rho v = J = \frac{I}{\text{area}} \\ \\ 
\frac{dW_{q}}{dt} = \int _{} E\cdot J \, d^{3}x 
\end{gather}
$$

Magnetic field don't add or subtract energy, they just turn the charges around. 

Some math?.... Need Maxwell's Equations. Let's figure out how we can reexpress
$$
\begin{gather}
E\cdot J
\end{gather}
$$
we have
$$
\begin{gather}
\frac{1}{\mu_{0}} \nabla \times B= J+\epsilon_{0} \frac{ \partial E }{ \partial t } 
\end{gather}
$$
so, 
$$
\begin{gather}
E\cdot J = \frac{1}{\mu_{0}} \nabla \times B-\left( J+\epsilon_{0} \frac{ \partial E }{ \partial t }  \right) \\ \\
\end{gather}
$$
In general we have this math relationship, 
$$
\begin{gather}
\nabla \cdot(E\times B) = B \cdot(\nabla \times E)-E\cdot(\nabla \times B) \\ \\
\end{gather}
$$
So what we find is,
$$
\begin{gather}
E \cdot(\nabla \times B) = -B \cdot \frac{ \partial B }{ \partial t } - \nabla \cdot(E\times B)  \\ \\ 
\frac{ \partial  }{ \partial t }  B^{2} = \frac{1}{2} B \cdot \frac{ \partial B }{ \partial t} \hspace{.5cm} \frac{ \partial  }{ \partial t } E^{2} = \frac{1}{2} E\cdot \frac{ \partial E }{ \partial t } 
\end{gather}
$$
Thus we get (finally?),
$$
\begin{gather}
E\cdot J = -\frac{1}{2}\frac{ \partial  }{ \partial t } \left( \epsilon_{0}E^{2}+ \frac{1}{\mu_{0}}B^{2} \right)- \frac{1}{\mu_{0}}\nabla \cdot(E\times B) \\ \\ 
= - \frac{ \partial W_{EB} }{ \partial t } - \nabla \cdot S
\end{gather}
$$
Thus putting this value back into our original integral we have, 
$$
\begin{gather}
\frac{dW_{q}}{dt} = - \frac{ \partial W_{EB} }{ \partial t } - \int S \cdot da \hspace{.5cm}\leftarrow  \text{Poynting's Theorem}
\end{gather}
$$
Where the first term on the right is directly from fields and the other one is the flux of electromagnetic energy through surface. It represents the conservation of electromagnetic energy. 