![[Pasted image 20240206112521.png|center|600]]

Announcements: 
- Lab: electrostatics

$E=\frac{1}{4\pi\epsilon0} \frac{Q}{r^{2}}$

$$\int _{1}^2 E\, dl = \int _{1}^2 E\, dr = \int _{1}^2 E \, dr = \frac{Q}{4\pi\epsilon_{0}}\int _{1}^2 \frac{1}{r^{2}}\, dr =\frac{Q}{4\pi\epsilon_{0}}(1/r)|_1 ^2 = \frac{Q}{4\pi\epsilon_{0}}\left( \frac{1}{r_{2}}-\frac{1}{r_{1}} \right) $$
$$
\begin{gather}
\phi_{21} = - \int _{1}^2 E \, dl  \\ \\ 
\text{where} \hspace{.2cm} F=qE, \hspace{.2cm} W = q\phi
\end{gather}
$$
![[Pasted image 20240206114558.png|center|300]]

Properties of $\phi$: 
- $\phi_{21}\equiv \int E \, dl$
- path independent 
- $\underbrace{ \oint }_{ \text{closed path} \hspace{.2cm} } E\cdot dl =0$
	- $\underbrace{ \oint }_{ a\mathrm{Re}a } \nabla \times E \cdot da = 0$ which is Stokes Theorem. 
- Thus $\nabla \times E = 0$ 
- For any vector function $E$ $\nabla \times(\nabla \phi)\equiv 0$. Thus we can say $E = -\nabla \phi$ 
![[Pasted image 20240206115319.png|center|300]]


Superposition:
$$
\begin{gather}
\phi(r) = \phi(x,y,z) = \int \frac{\underbrace{ \rho(x',y',z') }_{ dq }}{4\pi\epsilon_{0}r} \, dv 
\end{gather}
$$
##### Examples:

1. Semi circle of charge

$$
\begin{gather}
\oint E \cdot da = \frac{Q_{in}}{\epsilon_{0}} 
\end{gather}
$$
![[Pasted image 20240206120219.png|center|300]]

What is $E$?
Well $Q = \rho d =\lambda dl$ and $\Lambda=\frac{Q}{\pi a}$ and $dq = \lambda dl = \frac{Q}{\pi a} a d\theta$. Thus we have that $E_{x} - \int dE_{x} \,= \frac{kQ}{\pi a}a \int_{0}^\pi \frac{d\theta}{a}\sin\theta \, =$ Thus $E = E_{x}\hat{x} = \frac{2}{\pi}\frac{kQ}{a^{2}}$

pic
We have that $d\phi = \frac{kdq}{a}=\frac{kQ}{\pi a^{2}}\int  \, dl =$
$$
\begin{gather}
\frac{kQ\pi a}{\pi a} \frac{1}{a} = \frac{kQ}{a} =\phi
\end{gather}
$$

pic

Thus we have that 
$$
\begin{gather}
E =E_{z} \hat{z} = \frac{kQ}{(a^{2}+z^{2}) \frac{z}{\sqrt{ (a^{2}+z^{2}) }}} = \frac{kQz}{(a^{2}+z^{2})^{3/2}} \\ \\ 
E(0)= 0 \hspace{.5cm} \\ \\ 
 
 \text{when} \hspace{.2cm}z\gg a \\ \\ 
  E \rightarrow \frac{kQ}{z^{2}}
\end{gather} \\ \\

$$
Now we think about the potential: 
$$
\begin{gather}
\phi(z) = \frac{kQ}{\sqrt{ a^{2}+z^{2} }}
\end{gather}
$$
Thus we extract the electric field from the potential
$$
\begin{gather}
E = -\nabla \phi = -\frac{ \partial  }{ \partial t } \phi \\ \\ 

\text{Do derivative stuff} \hspace{.2cm}
\end{gather}
$$
![[Pasted image 20240206123517.png|center]]

$$
\begin{gather}
dE_{z} = \frac{kdQz}{(a^{2}+z^{2})^{3/2}} \\ \\ 

dQ = \sigma (2\pi rdr) \\ \\ 

E_{z} = \int _{0}^a \frac{\sigma(2\pi r dr)z}{(r^{2}+z^{2})^{3/2}} \, = \frac{2\pi\sigma z}{4\pi\epsilon_{0}}\left[ -\frac{1}{\sqrt{ z^{2}+ r^{2} }} \right]_{r=0}^{r=a} = \frac{\sigma}{2\epsilon_{0}}\left[ 1-\frac{z}{\sqrt{ z^{2}+a^{2} }} \right] \\ \\

E(0) = \frac{\sigma}{2\epsilon_{0}}: \hspace{.5cm} z\ll a \\ \\ 

z\gg a: \hspace{.5cm} E_{z}(z\rightarrow \infty) = kQ \frac{1}{\epsilon_{0}}


\end{gather}
$$
