#### Fourier Series

Periodic functions on $\mathbb{R}$ with period 1
- For the most part an $L^{2}$ - theory (squared integralize function)

$$
\begin{gather}
\begin{cases}
\cos(2\pi nx)  \hspace{.5cm}\leftarrow\text{even function} \hspace{.2cm}\\
\sin(2\pi nx) \hspace{.5cm}\leftarrow\text{odd fucntion} \hspace{.2cm}\\
\end{cases} \\ \\

\text{another system} \hspace{.2cm} e^{ 2\pi \sqrt{ -1 }nx } \hspace{.5cm} n\in \mathbb{Z}

\end{gather}
$$
Those are two different families:
 - we'll call the second one 
 $$
\begin{gather}
e_{n}(x) = e^{ 2\pi \sqrt{ -1 }nx } \\ \\
\int _{0}^1 \underbrace{ e_{n}(x) e_{m}(x) }_{ e^{ 2\pi \sqrt{ -1 }(n-m) x} }\, dx  = \begin{cases}
0 \hspace{.5cm} if \hspace{.2cm} n\neq m \\
1 if \hspace{.2cm} n=m
\end{cases}
\end{gather}
$$
- for the first case, if you integrate them and they're different, you get zero: 
$$
\begin{gather}
\int _{0}^1 \underbrace{ \cos(2\pi nx)\sin(2\pi nx) }_{\frac{1}{2}( \sin(2\pi(n+m)x)+\sin(2\pi(m-n)) })\, dx  = 0 \\ \\

\int _{0}^1 \cos(2\pi nx)\cos(2\pi mx) \, d = 0 \hspace{.5cm}\ if \hspace{.2cm} n\neq m \\ \\ 
= \int _{0}^1 \sin(2\pi nx)\sin(2\pi mx) \, dx  \\ \\ 

\int _{0}^1 \cos ^{2}(2\pi nx) \, d = \frac{1}{2} = \int _{0}^1 \sin ^{2}(2\pi nx) \, dx 
\end{gather}
$$
Recall (finite dimensional) vector spaces with inner product" 
$$
\begin{gather}
(. |. ): V \times V \rightarrow V \\ \\
(V_{1} | w_{1} +w_{2}) = (v|w_{1}) + (v|w_{2}) \\ \\
(v_{1} + v_{2}| w) = (v_{1}|w) + (v_{2}|w) \\ \\ 
(cv|w) = c(v|w) \\ \\ 
\end{gather}
$$
$$
\begin{gather}
W \in V \\ \\ 
proj_{w}: \hspace{.5cm}V\rightarrow W \\ \\ 
\text{orthogonal projection} \hspace{.2cm} \\ \\ 
\text{Suppose W is the finite dimensional} \hspace{.2cm} \\ \\
\end{gather}
$$
(Consider periodic functions: on $\mathbb{R} / \mathbb{Z}$, square integral) = $L^{2}(\mathbb{R} / \mathbb{Z})$ with inner product five by 
$$
\begin{gather}
(f|g) = \int  _{0}^1 f(x) \bar{g(x)} \, dx  \\ \\
\lvert (f|g) \rvert \leq \lvert | f|\rvert \cdot \lvert | g|\rvert  \hspace{.5cm}\leftarrow \text{Cauchy-Schwartz inequality} \hspace{.2cm}\\ \\

\lvert | g|\rvert = \int _{0}^1 g(x) \bar{(g(x))}\, dx 
\end{gather}
$$

Consider:
$$
\begin{gather}
e^{ 2\pi \sqrt{ -1 }nx }_{-n\leq n\leq N} \hspace{.5cm} f \in L^{2}(\mathbb{R} / \mathbb{Z}) \\ \\
proj_{span\mathbb{C} e^{ 2\pi \sqrt{ -1 }nx }} (f) \leftarrow-N \leq n\leq N \\ \\ 

\sum_{-N \leq n\leq N} (f|e^{ 2\pi \sqrt{ -1 }nx })e^{ 2\pi \sqrt{ -1 }nx } = \int _{0}^1 \underbrace{ f(x) e^{ -2\pi \sqrt{ -1 }nx } }_{ C_{n}(f) } \, dx \\ \\ 
f \rightarrow \sum_{n \in \mathbb{Z}} c_{n} e^{ 2\pi \sqrt{ -1 }nx } \\ \\
c_{n}(f) = \int_{0}^1  f(x) e^{ -2\pi \sqrt{ -1 }nx } \, dx  \\ \\ 
\text{suppose we really like sin,cos} \hspace{.2cm} \\ \\ 
\cos(nx)_{o\leq n\leq N} , \sin(x)_{1\leq n\leq N} \\ \\ 
f \rightarrow \sum_{n \in \mathbb{Z}} c_{n} e^{ 2\pi \sqrt{ -1 }nx }  = A_{0} + \sum_{n\geq 1} A_{n}\cos(2\pi nx) + \sum_{n\geq 1}\sin(2\pi nx) \\ \\
f \rightarrow \sum_{n \in \mathbb{Z}} c_{n} e^{ 2\pi \sqrt{ -1 }nx } = C_{n}e^{ 2\pi \sqrt{ -1 }nx }+C_{n}e^{ -2\pi \sqrt{ -1 }nx } \\ \\
= C_{n}[\cos(2\pi nx)+\sqrt{ -1 }\sin(2\pi nx)] + C_{n}[\cos(2\pi nx)-\sqrt{ -1 }\sin(2\pi nx)] \\ \\

\end{gather}
$$
EBT!
$$
\begin{gather}
= \underbrace{ (C_{n}+C_{-n}) }_{ A_{n} }\cos(2\pi nx)+\underbrace{  \sqrt{ -1 }(C_{n}-C_{-n}) }_{ B_{n} }\sin(2\pi nx) \\ \\
\text{then} \hspace{.2cm} A_{0} = \int _{0}^1 f(x) \, d \hspace{.5cm} \\ \\ 
for\hspace{.2cm} n\geq 1  \hspace{.5cm} A_{n} = 2(f|\cos(2\pi nx)) \\ \\ 
for\hspace{.2cm} B_{n} = 2(f|\sin(2\pi nx)) \\ \\
\end{gather} 
$$
Suppose $f(x)$ is periodic on $\mathbb{Z}$ continously differentiable. Our question is , does
$$
\begin{gather}
S_{N}(x) = \sum_{_{N\leq n \leq N}} c_{n}(f) e^{ 2\pi nx } \hspace{.2cm} \text{converge to } \hspace{.2cm} \\ \\ 
\text{f(x) for every x?} \hspace{.2cm} \text{where} \hspace{.2cm}\int _{0}^1 f(y) e^{ -2\pi \sqrt{ -1 }nx } \, dy \\ \\
S_{n}(x) \int_{0}^1 f(y) \underbrace{ \left[ \sum_{\lvert n \rvert\leq N} e^{ 2\pi \sqrt{ -1 }n(x-y) } \right] }_{ K_{N}(x-y) } \, dx \\ \\ 
\text{where} \hspace{.2cm} \underbrace{ K_{n}(\theta) }_{ \text{Dirichlet Kernal} \hspace{.2cm} } = \sum_{n= -N}^N e^{ 2\pi \sqrt{ -1 }n\theta } \\ \\
= \sum_{n=-N}^N e^{ 2\pi \sqrt{ -1 }n\theta } = e^{ 2\pi \sqrt{ -1 }N\theta } \cdot \sum_{n=0}^{2N} e^{ 2\pi \sqrt{ -1 }n\theta }\\ \\

\text{where} \hspace{.2cm} \sum_{n=0}^{2N} e^{ 2\pi \sqrt{ -1 }n\theta } = \frac{e^{ 2\pi(2N+1)\theta }-1}{ e^{ 2\pi \sqrt{ -1 }\theta }-1}
\end{gather}
$$
EBT!

$$
\begin{gather}
= \frac{\sin\left( 2\pi\left( N+\frac{1}{2} \right)\theta \right)}{\sin(\pi\theta)}
\end{gather}
$$
Thus
$$
\begin{gather}
f(x) -  S_{n}(x) \\ \\ 
\text{thus} \hspace{.2cm} \int _{0}^1 K_{n}\theta \, d\theta = 1 \\ \\ 
S_{N}(x) - f(x) = \int _{0}^1 K_{N}(x-y)f(y) \, dy - \int_{0}^1 f(x) K_{N}(x) \, dx  \\ \\ 

\end{gather}
$$