We'll start with the method Spherical Means (reduced to wave equation of dimension 1) to prove the Kircchoff's formula. Kircchoff's formula gives an explicit formula for the initial value problem of the wave equation in dimension three. 
$$
\begin{gather}
u_{tt} = u_{x x}+u_{yy}+u_{zz} \\ \\ 
u(x,y,z,0) = \phi(x,y,z) \hspace{.5cm}u_{t}(x,y,z,0) =  \psi(x,y,z)
\end{gather}
$$
Suppose you have smooth function $u(x,y,z,t)$ is a smooth function on $\mathbb{R}^{3} \times \mathbb{R}$. Now consider the function 
$$
\begin{gather}
r \geq 0  \\ \\ 
Iu(\vec{x},r,t) = \hspace{.2cm}\text{the average value of} \hspace{.2cm}u(\vec{x},t)\hspace{.2cm}\text{ on the sphere }\hspace{.2cm} S(\vec{x},r,t) = \begin{cases}
(\vec{y},t)=\lvert \vec{y}-\vec{x}  \rvert = r
\end{cases}
\end{gather}
$$
we can rewrite this as 
$$
\begin{gather}
\frac{1}{4\pi}\iint_{z\in S_{1}} u(\vec{x}+r\vec{z},t) \, dS_{z,1} 
\end{gather}
$$
where $S_{1}$ is the unit sphere in $\mathbb{R}^{3}$. We will see that if $u(\vec{x},t)$ satisfies the wave equation, then the function $Iu$ satisfies a second order variant of the wave equation in $(r,t)$. Suppose 
$$
\begin{gather}
\triangle I(u)(\vec{x},r,t)
\end{gather}
$$
we do the chain rule such that
$$
\begin{gather}
\frac{ \partial u }{ \partial x_{1} } =\frac{ \partial u }{ \partial x_{1} } ( )
\\ \\ 
\text{where} \hspace{.2cm}\vec{x}= (x_{1},x_{2},x_{3}) \hspace{.2cm}\vec{z}= (z_{1},z_{2},z_{3}) \\ \\ 
g(x,y,z) \\ \\ 

f(x,y,z,w,t,v) = g(x+w,y+t,z+v) \\ \ \
\frac{ \partial f }{ \partial x }  = g_{1}\left( \frac{ \partial (x+w) }{ \partial x }  \right)+g_{2}\frac{ \partial (y+t) }{ \partial x } +g_{3}\frac{ \partial (z+v) }{ \partial x } 
\end{gather}
$$
so we have 
$$
\begin{gather}
f(\vec{x},r,\vec{z},t) = u(\vec{x}+r\vec{z},t) \\ \ \
\frac{ \partial f }{ \partial x_{1} }(\vec{x},r,\vec{z},t) = \frac{ \partial u }{ \partial x_{1} } (\vec{x}+r\vec{z},t)
\end{gather}
$$

Now let's think about the relation between spherical average over balls. Suppose we want to compute
$$
\begin{gather}
Ju(\vec{x},r,t)
\end{gather}
$$
where $Ju$ is the average of $u(\vec{y},t)$ of the ball with $\begin{cases} \lvert \vec{y}-\vec{z} \rvert\end{cases}\leq r$}. This is 
$$
\begin{gather}
= \frac{3}{4\pi r^{3}}\int _{0}^r 4\pi(Iu)(\vec{x},\rho,t) \rho^{2} \, d\rho
\end{gather}
$$
Now we have 
$$
\begin{gather}
J(\triangle u)(\vec{x},r,t) =\frac{3}{r} \frac{ \partial  }{ \partial r } (Iu)(\vec{x},r,t)\\ \\
\triangle = \nabla \cdot(\nabla u) \\ \\ 
= \frac{3}{4\pi r^{3}} \iint_{S(\vec{x},r)}( \nabla u) \frac{\vec{y}-\vec{x}}{r} \, dS_{\vec{y}}(\vec{x},r)
\end{gather}
$$
where $\vec{y}$ with $\lvert \vec{y}-\vec{x} \rvert = r$. Now, how is this related to $Iu$? Well, 
$$
\begin{gather}
(Iu)(\vec{x},r,t) = \frac{1}{4\pi r^{2}}\iint_{\vec{y} \in S(\vec{x},r)} u(\vec{y},t) \, d_{\vec{y}}S(\vec{x},r) \\ \\ 

\frac{ \partial  }{ \partial r } (Iu)(\vec{x},r,t)= \frac{1}{4\pi}\iint_{z\in S_{o,1}} u(\vec{x}+r\vec{z},t) \, dS(0,1) \\ \\ 
\frac{ \partial  }{ \partial r } (Iu)(\vec{x},r,t) = \frac{1}{4\pi} \iint_{z \in S(0,1)} \nabla u(\vec{x}+y\vec{z}) \cdot \vec{z}\, d_{z}S(0,1) 
\end{gather}
$$
So now we see 
$$
\begin{gather}
 (Iu)(\vec{x},r,t) = \frac{1}{4\pi r^{2}}\iint_{\vec{y} \in S(\vec{x},r)} u(\vec{y},t) \, d_{\vec{y}}S(\vec{x},r) \frac{\cdot_{1}}{r^{2}} = \\ \\ 
\frac{3}{4\pi r}Iu(\vec{x},r,t)
\end{gather}
$$
Now let's suppose we have another function $v$, 
$$
\begin{gather}
J(v)(\vec{x},r,t) = \int _{0}^r 4\pi\rho^{2}(Iv)(\vec{x},r,t) \cdot d\rho \\ \\
4\pi r^{2}(Iv)(\vec{x},r,t) = \frac{ \partial  }{ \partial r } (Jv)(\vec{x},r,t) \\ \\ 
(Iu)(\vec{x},r,t) = \frac{1}{4\pi r^{2}} \frac{ \partial  }{ \partial r } (Ju)(\vec{x},r,t)
\end{gather}
$$
We have that 
$$
\begin{gather}
r\cdot(Iu)(\vec{x},r,t) 
\end{gather}
$$
satisfies the wave equation in $r,t$ i.e., 
$$
\begin{gather}
\left( \frac{ \partial^{2} }{ \partial t^{2} } -c^{2} \frac{ \partial^{2} }{ \partial r^{2} }  \right)(r\cdot (Iu)(\vec{x},r,t)) = 0
\end{gather}
$$
if $u(\vec{x},r,t)$ satisfies the wave equation. 
