##### Divergence Theorem in higher dimensions

Why discussing this: Wave equation in dimension 3
$$
\begin{gather}
(u_{tt}-c^{2}\triangle u)u = -c^{2} \nabla \cdot(u_{t}\cdot \nabla u)+ \underbrace{ \left( \frac{1}{2}u_{t}^{2}+\frac{1}{2}\lvert \nabla u \rvert^{2} \right) }_{ \text{energy density} }
\end{gather}
$$
If $u$ satisfies $u_{tt}-c^{2} \triangle u = 0$ and $u$ decays rapidly in $(x_{1},x_{2},x_{3})$. e.g $\leq\cdot \lvert \lvert x \rvert \rvert^5$. We then discover
$$
\begin{gather}
\frac{d}{dt}\int _{\mathbb{R}^{3}} \left( \frac{1}{2}u_{t}^{2}+\frac{1}{2}\lvert \nabla u \rvert^{2} \right) \, d^{3}x =0
\end{gather}
$$
We notice we can think of the right hand side of the first math equation as a divergence in $\mathbb{R}^4$. Causality follows from Kirchhoff's formulas such that the solution $u(\mathbf{x},t)$ defined on $\mathbb{R}^{3}\times \mathbb{R}$ depends only on
$$
\begin{gather}
u| y \in \mathbb{R}^{3}, \hspace{.5cm}ct-\epsilon<\lvert y-x \rvert <ct+\epsilon \\ \\ 
u_{t} | y \in \mathbb{R}, \hspace{.2cm} \lvert y-x \rvert = ct
\end{gather}
$$
![[Pasted image 20240410122534.png|center]]

Furthermore
$$
\begin{gather}
t=t_{2}>0, \hspace{.5cm}\lvert y-x \rvert= c(t_{1}-t_{2})
\end{gather}
$$
We now state the divergence of a vector field in $\mathbb{R}^4$ with respect to $t$
$$
\begin{gather}
\frac{1}{2}u_{t}^{2}+ \frac{1}{2} \lvert \nabla u \rvert^{2}, -c^{2}u_{t} u_{x},-c^{2}u_{t}u_{y},-c^{2}u_{t}u_{z}
\end{gather}
$$

Focusing specifically on the top and bottom disks of the cone we have 
$$
\begin{gather}
\text{energy integral to for t=0} = \text{(energy integral for} \hspace{.2cm}t_{1})+ \int_{\text{the collar}} (\text{the vector field on}) \hspace{.2cm} \mathbb{R}^{3}\times \mathbb{R} \, dx 
\end{gather}
$$
##### Higher dimensional integral with signs (not sums lol)

The standard treatment (in math) through "differential forms". Let's begin with $\mathbb{R}^{3}$. Dimension wise we have three types of integrals
- line integrals
- surface integrals
- and integrals of a solid in $\mathbb{R}^{3}$
For the last bullet point, we usually see integrals like
$$
\begin{gather}
\iiint f(x,y,z)dx\lambda dy\lambda dz  \\ \\
dx\lambda dz\lambda dy = -dx\lambda dy\lambda dz \\ \\ 
dz \lambda dx\lambda dy = dx\lambda dy\lambda dz
\end{gather}
$$
Now if we make a change of variables we have
$$
\begin{gather}
(x(u,v,w),y(u,v,w),z(u,v,w))
\end{gather}
$$
now the "with respect to" portion at the end of the integral becomes
$$
\begin{gather}
\left( \frac{ \partial x }{ \partial u } du+\frac{ \partial x }{ \partial v } dv+\frac{ \partial x }{ \partial w } dw \right), \\ \\ 
\left( \frac{ \partial y }{ \partial u } du+\frac{ \partial y }{ \partial v } dv+\frac{ \partial y }{ \partial w } dw \right),\left( \frac{ \partial z }{ \partial u } du+\frac{ \partial z }{ \partial v } dv+\frac{ \partial z }{ \partial w } dw \right),
\end{gather}
$$
So we have the determinant equal to 
$$
\begin{gather}
\det\left( \frac{\partial(x,y,z)}{\partial(u,v,w)} \right) 
\end{gather}
$$


So the integrand looks like after making the parametrization $\gamma=a$ parametrization of $C$ $\gamma:[a,b]\rightarrow\mathbb{R}^{3}$
$$
\begin{gather}
\int _{C} fdx+gdy+hdz = \int _{a}^b f(\gamma(t)) \frac{d\gamma}{dt} + g(\gamma(t)) \frac{d\gamma_{2}}{dt}+h(\gamma(t)) \frac{d\gamma_{3}}{dt}
\end{gather}
$$
Now suppose we integrate over the surface
$$
\begin{gather}
\int _{S} f_{1}dy\lambda dz+f_{2}dz\lambda dx+f_{3}dx\lambda dy  \\ \\
\gamma: \underbrace{ D }_{ \mathbb{R}^{2} }\rightarrow\mathbb{R}^{3} \hspace{.5cm}(\gamma_{1},\gamma_{2},\gamma_{3}) \rightarrow\text{a domain in} \hspace{.2cm}\mathbb{R}^{3}
\end{gather}
$$
where the first term is equal to 
$$
\begin{gather}
f_{1}dy\lambda dz = f_{1}(\gamma(t))\cdot\left( \frac{ \partial \gamma_{2} }{ \partial u_{1} } du_{1}+ \frac{ \partial \gamma_{2} }{ \partial u_{2} }du_{2}  \right)\lambda \left( \frac{ \partial \gamma^{3} }{ \partial u_{1} } du_{1}+ \frac{ \partial \gamma_{3} }{ \partial u_{2} } du_{2} \right) \\ \\ 
= \det \begin{pmatrix}
\frac{ \partial \gamma_{2} }{ \partial u_{1} } & \frac{ \partial \gamma_{2} }{ \partial u_{2} }  \\
\frac{ \partial \gamma_{3} }{ \partial u_{1} } & \frac{ \partial \gamma_{3} }{ \partial u_{2} } 
\end{pmatrix}
\end{gather}
$$
$$
\begin{gather}
df= \frac{ \partial f }{ \partial x_{1} } dx_{1}+ \frac{ \partial f }{ \partial x_{2} }dx_{2}+ \frac{ \partial f }{ \partial x_{3} } dx_{3} \\ \\
d(fdx+gdy+hdz) \\ \\ 
= df\lambda dx+dg\lambda dy+dh\lambda dz \\ \\
\text{where} \hspace{.5cm} df\lambda dx = \left( \frac{ \partial f }{ \partial x }dx+ \frac{ \partial f }{ \partial y } dy+\frac{ \partial f }{ \partial z } dz  \right)\lambda dx= - \frac{ \partial f }{ \partial y } dx\lambda dy+\frac{ \partial f }{ \partial z } dz\lambda dx \\ \\ 
\end{gather}
$$
The general stokes or divergent theorem takes the following form, 
$$
\begin{gather}
\iint _{\partial D} \alpha = \int _{D} d\alpha  \\ \\
dimD = m_{1} \hspace{.5cm}dim\partial D=m
\end{gather}
$$
where $\alpha$ is smooth on $D$. Look at the Micheal Spevack (?) book for further explanation. 

#### Bessel Functions
Bessel functions of the first kind and integral order

Bessel's ODE looks like
$$
\begin{gather} *
\frac{d^{2}u}{dx^{2}} + \frac{1}{x} \frac{du}{dx}+ \left( 1-\frac{\lambda^{2}}{x^{2}} \right)u=0 \\ \\ 
 \text{equivalently} \hspace{.2cm}\left[ \left( x \frac{d}{dx} \right)^{2}+(x^{2}-\lambda^{2}) \right]u=0 \\ \\ 
\end{gather}
$$
we have 
$$
\begin{gather}
x^\nu \cdot \sum_{n\geq 0}c_{n}x^n
\end{gather}
$$
where $\nu$ satisfies the second order algebraic equation (indicial equation). we have that 
$$
\begin{gather}
\lambda^{2}= \boxed{}
\end{gather}
$$
$J_{\nu}(x) =$ a power series in $x$ satisfying ($*$). $J_{n}(x)$ with explicitly coefficient in their power series 
$$
\begin{gather}
e^{ 1/2(x(t-t^{-1})) } = \sum_{n \in \mathbb{Z}} J_{n}(x) t^n \\ \\ 
e^{ 1/2(x(t-t^{-1})) } = e^{ (1/2)xt } \cdot e^{ (-1/2xt^{-1}) }
\end{gather}
$$
For more for information on Besssel's function look at the NIST handbook on mathematical functions.
https://dlmf.nist.gov/10 

Bowmen