#### Bessel Functions

Let's take a look at some gamma functions
$$
\begin{gather}
\Gamma(x) =  \int _{0}^\infty e^{ -t }t^x \, \frac{dt}{t}
\end{gather}
$$
which converges absolutely for $Re(x) >0$. We have that 
$$
\begin{gather}
\Gamma(n) = (n-1)! \hspace{.5cm} \forall n\geq 1 \hspace{.5cm} n=1,2,3,\dots
\end{gather}
$$
Bessel functions are often called cylindrical functions. Bessel's ODE
$$
\begin{gather}
(*)_{\upsilon}:\left[ \frac{d^{2}}{dx}+ \frac{1}{x} \frac{d}{x}\left( 1-\frac{\lambda^{2}}{x^{2}} \right) \right] y = 0
\end{gather}
$$
where $\lambda$ is a parameter. Thus we have, 
$$
\begin{gather}
\left[ \left( x \frac{d}{dx} \right)^{2}+x^{2}-\lambda^{2} \right]u = 0
\end{gather}
$$
in many situations, the previous equation is easier to deal with the earlier equivalent. For $\left( x \frac{d}{dx} \right)$ we have $x^\upsilon = \upsilon \cdot x^\upsilon$. The more common or easier Bessel ODE is when $\lambda$ is an integer, 
$$
\begin{gather}
\lambda \in \mathbb{Z} \rightarrow J_{n}(x): \text{satisfies} \hspace{.2cm} (*)_{n}
\end{gather}
$$
For Bessel function of the first kind with with integral $n$ order/index. They are best defined by the generating function
$$
\begin{gather}
e^{ 1/2 }x(t-t^{-1}) = \sum_{n \in \mathbb{Z}} J_{n}(x)t^n \\ \\ 
e^{ 1/2(xt) } e^{ -x/2t } = \sum_{k=0}^\infty \left( \frac{1}{2} \right) \frac{(xt)^k}{k!} \sum_{l=0}^\infty (-1)^l\left(  \frac{1}{2}\right)^l \frac{(xt^{-1})^l}{l!}
\end{gather}
$$
$J_{n}(x)$ is a coefficient of $t^n$ in the product 
$$
\begin{gather}
\sum_{n \in \mathbb{Z}} \sum_{k,l \geq 0} \frac{\left( (-1)^l \left( \frac{1}{2} \right)^l \cdot x^{k+1} \right)}{k!l!} t^n
\end{gather}
$$
where $k-l=n$. Thus we have the Bessel solution
$$
\begin{gather}
J_{n}(x) = \sum_{k-l=n} \frac{(-1)^l x^{k+1}}{2^{k+1} k!l!} \hspace{.5cm}k,l \geq 0
\end{gather} 
$$
now let's think about what this means. Let's say $n\geq 0$, 
$$
\begin{gather}
k = l+n \hspace{.5cm} k+l = n+ 2l
\end{gather}
$$
$$
\begin{gather}
J_{n}(x) = \sum_{l=0}^\infty \frac{(-1)^l \cdot x^{2l+n}}{2^{2l+n}l!(l+n)!} \\ \\ 
J_{n}(x)= \frac{x^n}{2^n n!} \sum_{l=0}^\infty (-1)^l \frac{x^{2l}}{2^{2l}l! \cdot(n+1)\dots (n+l)} \\ \\ 
\end{gather}
$$
The radius of convergence is $\infty$ and you can use the ratio test to show that $J_{n}(x)$ converges absolutely for all $x$. Want to check that $J_{n}(x)$ satisfies $(*)_{n}$. Let's use the generating function
$$
\begin{gather}
e^{ 1/2 }x(t-t^{-1}) = \sum_{n \in \mathbb{Z}} J_{n}(x)t^n \\ \\ 
\left( x \frac{d}{dx} \right) e^{ 1/2 (x(t-t^{-1}) )} = \frac{1}{2}x(t-t^{-1})e^{ 1/2(x(t-t^{-1})) } \\ \\ 
\left( x \frac{d}{dx} \right)^{2} e^{ 1/2 (x(t-t^{-1}) )} = \frac{1}{4}x^{2}(t-t^{-1})^{2} \cdot e^{ (1/2)x(t-t^{-1}) }+\frac{1}{2}x(t-t^{-1})\cdot e^{ (1/2) (t-t^{-1}) }
\end{gather}
$$
we do a similar thing for the operator $\left( t \frac{d}{dt} \right)$ 
$$
\begin{gather}
\left( t \frac{d}{dt} \right)e^{ (1/2) }x(t-t^{-1}) = \frac{1}{2}x(t+t^{-1}) e^{ (1/2)x(t+t^{-1}) } \\ \\ 
\left( t \frac{d}{dt} \right)^{2} e^{ (1/2)x(t+t^{-1}) } = \frac{1}{4}x^{2}(t+t^{-1})^{2} \cdot e^{ (1/2)x(t+t^{-1}) } + \frac{1}{2}x(t+t^{-1}) e^{ (1/2)x(t+t^{-1}) } \\ \\ 
= \frac{1}{4}x^{2}(t+t^{-1})^{2} e^{ (1/2)x(t+t^{-1}) }+ x^{2} e^{ (1/2)x(t+t^{-1}) } + \frac{1}{2}x(t+t^{-1})e^{ (1/2)x(t+t^{-1}) }
\end{gather}
$$
Thus we conclude, 
$$
\begin{gather}
\left[ \left( x \frac{ \partial  }{ \partial x }  \right)^{2}+x^{2}- \left( t \frac{ \partial  }{ \partial t }  \right)^{2} \right] e^{ (1/2)x(t+t^{-1}) } = 0
\end{gather}
$$
Thus $J_{n}(x)$ satisfies $(*)_{n}$ for all $n \in \mathbb{Z}$. Now we can change the signs $x,t$  in the generating function such that
$$
\begin{gather}
e^{ (1/2)(-x)(t^{-1}-t) } = \sum_{n\in \mathbb{Z}} J_{n}(-x)t^n = \sum_{n \in \mathbb{Z}}J_{n}(x)t^{-n} \\ \\ 
J_{-n}(x) = J_{n}(-x) = (-1)^n J_{n}(x)
\end{gather}
$$
$J_{n}(x)$ is even if $n$ is even and odd if $n$ is odd. 
$$
\begin{gather}
e^{ (1/2)xt(xt-1/xt) } = \sum_{n \in \mathbb{Z}} x^n J_{n}(x)t^n \\ \\ 
\end{gather}
$$
now we apply $\frac{d}{dx}$,
$$
\begin{gather}
e^{ (1/2)xt(x(xt-1/xt)) } = \sum_{n \in\mathbb{Z}} x^{n+1}J_{n}(x)t^{n+1} = \sum_{n \in \mathbb{Z}} \frac{d}{dx}(x^n J_{n}(x))t^n \\ \\ 
x^n J_{n-1}(x) = \frac{d}{dx}(x^n\cdot J_{n}(x)) \leftarrow \text{recursion!} \\ \\ 
\frac{d}{dx}(x^{-n}J_{n}(x)) = -x^{-n}J_{n+1}(x) \leftarrow \text{recursion!} \\ \\ 
\end{gather}
$$
Equivalently
$$
\begin{gather}
J_{n}'(x)+ \frac{n}{x} J_{n}(x) = J_{n-1}(x) \\ \\ 
J_{n}'(x) - \frac{n}{x}J_{n(x)} = -J_{n+1}(x) \\ \\ 
J_{n-1}'(x) + J_{n+1}(x) = \frac{2n}{x}J)n(x) \\ \\ 
J_{n-1}'(x) - J_{n+1}(x) = 2J_{n}'(x)
\end{gather} 
$$
for  $\alpha_{1},\alpha_{2}\dots$ we have positive zeros of $J_{0}(x)$ 
$$
\begin{gather}
0 = \int _{0}^1 xJ_{0}(\alpha_{i}x)\cdot J_{0}(\alpha_{j}x) \, dx \hspace{.5cm} if \hspace{.2cm}i \pm j
\end{gather}
$$


