Example: Linear Partial Differential Equations
- We'll use the "Method of Characteristcs"
-$$
\begin{gather}
U_{x} +2xy u_{y} = 0 \hspace{.5cm} \text{want to find the solution to this two variable equation} \\ \\ 
Note: \text{usually w ODE theres some kind of domain that gives you a particular solution. W PDEs, it could be the equation of a lesser order} \\ \\
\frac{dx}{1 } = \frac{dy}{2xy} \leftrightarrow  \begin{cases}
\frac{dx}{dt} = 1 \\
\frac{dy}{dt}= 2xy
\end{cases} \hspace{.5cm} \text{where y cannot be 0}\\ \\ 
\text{if} \hspace{.1cm} u(x,y) \hspace{.1cm} \text{is a solution and} \hspace{.1cm} \hspace{.1cm} (x(t), y(t)) \text{satisfies the ODE} \\ \\
2x dx = \frac{dy}{y} \\ \\ 
x^{2} +c = \log(y) \\ \\ 
c = \log \lvert y \rvert - x^{2}
Note: \hspace{.1cm} \text{ for and c, you get a solution curve.} \\ \\ 
\text{Thus} \hspace{.1cm} u(x,y) = f(\log \lvert y\rvert - x^{2})



\end{gather}
$$Notes: This is a very general form, and would depend on what $f$ is. The general solution of a PDE depends on a function, and other elements, rather than the ODE case that only depends on the ends of a domain (IVP)


#### Next up, we're gonna solve some easy PDEs:
- Wave equation in space dim = 1
$$
\begin{gather}
\frac{ \partial u }{ \partial t^{2} } - \frac{ \partial^{2}u }{ \partial x^{2} } \hspace{.5cm} \text{Linear, Homogenous, Second Order equation} \\ \\ 
\text{There are many many solution} \\ \\
\text{intial conditions:} \hspace{.1cm} \\ \\ \begin{cases} \\
u(x,0) = \phi(x) \\
\frac{ \partial u }{ \partial t } (x,0) = \psi(y)
\end{cases}
\text{initial conditions:} \hspace{.1cm} \text{Solve for} \hspace{.1cm} u(x,y) \hspace{.1cm}on \begin{cases}
(x,t) \hspace{.1cm} |\hspace{.1cm} x \hspace{.1cm} in \hspace{.1cm} \mathbb{R}, t\geq 0
\end{cases} \\ \\ 
Note: \text{ Important possible properties of a PDE:} \\ \\ 
\text{Space dim = 2 wave eq (can be used to model of a drum beat):} 
\frac{ \partial ^s }{ \partial t^{2} } - \frac{ \partial^{2} }{ \partial x^{2} } - \frac{ \partial^{2} }{ \partial y^{2} } = 0 \\ \\ 
(x,y) \hspace{.1cm} in \hspace{.1cm} D \hspace{.1cm} \text{bounded domain in} \hspace{.1cm} \mathbb{R}^{2} \hspace{.1cm} \text{with smooth boundary } \\ \\ 
u(x,y,t) \hspace{.1cm} \text{satisfies the PDE}  \\ \\ 
u(x,y,t) = 0 \hspace{.1cm} \text{if} \hspace{.1cm} (x,y) \hspace{.1cm} in \hspace{.1cm} b\underline{o}ary of D
u(x,y,0) =\phi(x,y) \hspace{.1cm} \text{where} \hspace{.1cm} \phi(x,y) \hspace{.1cm} \text{is given} \\ \\
\text{boudnary conditions:}\begin{cases}
\frac{ \partial u }{ \partial t }(x,y,0) = \psi(x,y)
\end{cases} \hspace{.1cm} \text{where} \hspace{.1cm} \psi(x,y) \hspace{.1cm} \text{is given} \\ \\
Note: \text{Solution depends continiously on the intial and boundary conditions or, "well composed"} 
\end{gather}
$$

--- 
$$
\begin{gather}
\frac{ \partial^{2} }{ \partial t^{2} } - \frac{ \partial^{2} }{ \partial x^{2} } = \left( \frac{ \partial  }{ \partial t } - \frac{ \partial  }{ \partial y }  \right) \left( \frac{ \partial  }{ \partial t } + \frac{ \partial  }{ \partial x } \right) \\ \\ 
\frac{ \partial^{2} }{ \partial y{ \partial z } } v = 0 \hspace{.5cm} v(y,z) \\ \\
\text{this says}: \frac{ \partial  }{ \partial y } \left( \frac{ \partial v }{ \partial z }  \right) = 0 \hspace{.1cm} \text{where f(z)} \hspace{.1cm} \text{such that} \hspace{.1cm}\frac{ \partial v }{ \partial z }  = f(z) \\ \\ 
v(y,z) = F(z) + g(y) \\ \\ 
Note: \hspace{.1cm} \text{functions in one varible, g(y) and F(z) such that} \hspace{.1cm} v(y,z) = g(y) + F(z) \\ \\ 
\underline{want} \hspace{.5cm} \begin{cases}
1. \frac{ \partial  }{ \partial y }  = \frac{ \partial  }{ \partial t } - \frac{ \partial  }{ \partial x } \hspace{.1cm} = \frac{ \partial t }{ \partial y } \frac{ \partial  }{ \partial t } + \frac{ \partial x }{ \partial y }  \frac{ \partial  }{ \partial x }  \\
2. \frac{ \partial  }{ \partial z  } =  \frac{ \partial  }{ \partial t } + \frac{ \partial  }{ \partial x }  = \frac{ \partial t }{ \partial z } \frac{ \partial  }{ \partial t } + \frac{ \partial x }{ \partial z }  \frac{ \partial  }{ \partial x } 
\end{cases} \\ \\ 
\text{Need/want} \begin{cases}
\frac{ \partial t }{ \partial y  } = 1, \hspace{.5cm} \frac{ \partial x }{ \partial y } =1  \\
\frac{ \partial t }{ \partial z } =1, \hspace{.5cm} \frac{ \partial x }{ \partial z } = 1 \\ 
\end{cases} \\ \\ 

\text{solution}: \begin{cases}
t = y+z \\
x = -y + z \\
\end{cases} \\ \\ 
\sum \hspace{.1cm}\text{functions F,G in one variable such that } u(x,t) = f\left( \frac{t-x}{2} \right) + G\left( \frac{t+x}{2} \right) = f(x-t) + g(x-t) \\ \\ 
\text{two functions of one variable} \\ \\ 
\underline{General \hspace{.1cm} Solution} = u(x,t) = f(x+t)+g(x-t) \text{Note: just by convetion for the +,-}
\end{gather}
$$

So if we compose this condition on the following function 
$$
\begin{gather}
u(x,t) = f(x+ct) + g(x-ct) \\ \\ 
\text{we determine f and g in terms of} \hspace{.1cm} \phi \hspace{.1cm} \text{and} \hspace{.1cm} \phi  \\ \\ 
\begin{cases} \\ 
u(x,0) = \phi(x) \leftrightarrow f(x) + g(x) = \phi(x) \\
\frac{ \partial u }{ \partial t } (x,0) = \psi(y) \leftrightarrow cf'(x) - cg'(x) = \psi \\
\end{cases} \\ \\ 
\text{where the first line} \\ \\ 
\begin{cases}
f'(x) + g'(x) = \phi(x) \\
cf'(x) - cg'(x) = \psi(x) \\
\end{cases} \\ \\
\text{ and the second is} \hspace{.1cm} f'(x) = \frac{\phi'(x) + \frac{1}{c}\psi(x)}{2} \hspace{.1cm} \text{and} \hspace{.1cm} g'(x) = f'(x) = \frac{\phi'(x) - \frac{1}{c}\psi(x)}{2} \\ \\ 
\text{ where} u(x,t) =  \frac{1}{2}[phi]
\end{gather} \\ \\

$$
