#### Bessel Functions
We recall, 
$$
\begin{gather}
e^{ (1/2)x(t-t^{-1}) } = \sum_{n \in \mathbb{Z}} J_{n}(x)t^n \\ \\ 
J_{n}(x) =  \sum_{k=0}^\infty(-1)^k \frac{\left( \frac{x}{2} \right)^{n+2k}}{(n+k)!k!} \hspace{.5cm}n\geq 0
\end{gather}
$$
We know that if $J_{n}(x)$ is odd or even then $n$ is odd or even. $J_{n}(x)$ has radius of convergence equal to infinity. We have the following property
$$
\begin{gather}
J_{n}(-x) = J_{-n}(x)=(-1)^n J_{n}(x)
\end{gather}
$$
We can rewrite $J_{n}(x)$, 
$$
\begin{gather}
J_{n}(x) = \frac{1}{n!}\left( \frac{x}{2} \right)^n(1+ \dots)
\end{gather}
$$
What happens when $x\rightarrow\infty$, 
$$
\begin{gather}
\lim_{ x \to \infty } \frac{J_{n}(x)}{\left( \frac{2}{\pi} \right)^{1/2}\frac{1}{\sqrt{ x }}\cos\left( x-\frac{n\pi}{2}-\frac{\pi}{4} \right)}=1
\end{gather}
$$
Recursion relations - trying to relate the derivates of the Bessel functions to neighboring Bessel functions. 
$$
\begin{gather}
\frac{d}{dx}(x^n)J_{n}(x) = x^n J_{n-1}(x) \\ \\ 
\frac{d}{dx}(x^{-n}J_{n}(x)) = -x^{-n}J_{n-1}(x)
\end{gather}
$$
equivalently this gives us
$$
\begin{gather}
J_{n}'(x)+ \frac{n}{x}J_{n}(x) = J_{n-1}(x)\\ \\ 
J_{n}'(x) - \frac{n}{x}J_{n}(x) = J_{n+1}(x)  \\ \\ 
J_{n-1}(x)+J_{n-1}(x) = \frac{2n}{x}J_{n}(x) \\ \\
J_{n-1}(x)-J_{n-1}(x) = 2J_{n}'(x)
\end{gather} 
$$
Where the first set of two equations are equal to the next. 

##### Orthogonality 
of Bessel Functions. 
$$
\begin{gather}
\left[ \left( x \frac{d}{dx} \right)^{2}+(x^{2}+n^{2}) \right]J_{n}(x) = 0
\end{gather}
$$
let $\alpha$ be a number any number (real or complex) such that 
$$
\begin{gather}
u(x) = J_{0}(\alpha x)
\end{gather}
$$
which satisfies 
$$
\begin{gather}
\left[ x^{2}\left( \frac{d}{dx} \right)^{2}+x \frac{d}{dx}+x^{2} \right]J_{0}(x) = 0 \\ \\ 
\left[ \left( \frac{d}{dx} \right)^{2}+\frac{1}{x} \frac{d}{dx}+1 \right]J_{0}(x) =0 
\end{gather}
$$
thus
$$
\begin{gather}
\left( x \frac{d}{dx} \right)^{2}u(x) = \alpha^{2}\left( \left( x \frac{d}{dx} \right)J_{0} \right) (\alpha x) \\ \\ 

\left[ \left( x \frac{d}{dx} \right)^{2}+\alpha^{2}x^{2} \right]u =0 \\ \\ 

\left( x \frac{d}{dx} \right)^{2}

\end{gather}
$$

Where we have the following ODE
$$
\begin{gather}
xu'' + u'+ \alpha^{2}xu \\ \\ 
v(x)  = J_{0}(\beta x) \\ \\ 
xv'' +v'+ \beta^{2}xu = 0
\end{gather}
$$
we can multiply the first equation by $v$ and the last one by $u$ to get, 
$$
\begin{gather}
x\underbrace{ (u''v-uv'') }_{ \frac{d}{dx(u'v-u'v)} }+(u'v-uv')+(\alpha^{2}-\beta^{2})xuv \\ \\ 
= \frac{d}{dx} [x(u'v-uv')] + (\alpha^{2}-\beta^{2})xuv
\end{gather}
$$
This tells us that if we integrate 
$$
\begin{gather}
(\alpha^{2}-\beta^{2})\int x^{2}uv \, dx = x(uv'-uv') 
\end{gather}
$$
suppose that $\alpha,\beta>0$ and $J_{0}(\alpha)=0$ = $J_{0}(\beta)=0$, 
$$
\begin{gather}
(\alpha^{2}-\beta^{2})\int _{0}^1 x^{2}J_{0}(\alpha x)J_{0}(\beta x) \, dx = 0 \\ \\ 


\end{gather}
$$
Now what about the case when $\alpha=\beta$ 
$$
\begin{gather}
xu''+u'+\alpha xu=0
\end{gather}
$$
we can multiply the that equation by $2xu'$ such that, 
$$
\begin{gather}
2x^{2}u'u''+2x^{2}u'^{2}+ 2xu'\alpha xu = 0 \\ \\ 
= \frac{d}{dx} (x^{2}\cdot(u')^{2})+ \frac{d}{dx}(\alpha^{2}2x^{2}\cdot u^{2})-2\alpha^{2}xu^{2}=0
\end{gather}
$$
We know that $u(1)\equiv_{0}$ and the last equation at $x=0$ is zero. Now we want to look at the following integral, 
$$
\begin{gather}
2\alpha^{2} \int _{0}^1 xJ_{0}(\alpha x) \, dx 
\end{gather}
$$
So we have 
$$
\begin{gather}
u'(1)^{2}= \alpha J_{0}'(\alpha)^{2} =\alpha J_{1}(x)^{2}
\end{gather}
$$
Try to solve a boundary value problem for the 2 dimension wave equation for a disk with a radius $a>0$. This will be an application of Bessel functions. Assume that $c=1$. We have, 
$$
\begin{gather}
\left( \frac{ \partial  }{ \partial t^{2} }- \triangle _{\mathbb{R}^{2}}  \right)u = 0 \hspace{.5cm} u(x,y,t)
\end{gather}
$$
The most natural coordinate system to use is polar coordinates. We write the laplacian in polar coordinates, 
$$
\begin{gather}
\triangle_{\mathbb{R}^{2}} =r^{-2} \left( r \frac{d}{dr} \right)^{2} + r^{-2} \frac{ \partial^{2} }{ \partial \theta^{2} } 
\end{gather}
$$
We want to find the product relationship of the form $R(r),\theta(\theta),T(t)$ such that, 
$$
\begin{gather}
0= \frac{1}{R\cdot\theta \cdot T} \left( \frac{ \partial  }{ \partial t^{2} } -\triangle \right) = \frac{\left( \frac{rd}{dr} \right)^{2}R}{r^{2}R}+ \\ \\ 
\frac{\frac{d^{2}}{d\theta^{2}}\theta_{f}}{\theta_{f}} + \frac{\frac{d^{2}}{dt^{2}}T}{T}= 0
\end{gather}
$$
Where $\theta_{f}$ is a function of theta that I cannot remember. 