##### Legendre Polynomials

$$
\begin{gather}
P_{n} = (P_{n}^o)
\end{gather}
$$
where $P_{n}$ is a polynomial of $n$ degree. IT has associated Legendre polynomial $P_{n}^m$ where $P_{n}=P_{n}^o$. We have the generation function for Legendre Polynomials
$$
\begin{gather}
\frac{1}{\sqrt{ (1-2t\zeta+t^{2}) }} = \sum_{n=0}^\infty P_{n}(\zeta)t^n \hspace{.5cm}(1)
\end{gather}
$$
In general, we can reduce this function by methods from single variable calculus, 
$$
\begin{gather}
(1+x)^\alpha = \sum_{n=0}^\infty \begin{pmatrix}
\alpha \\
n
\end{pmatrix}x^n
\end{gather}
$$
so we can substitute the second equation using, 
$$
\begin{gather}
\begin{cases}
\alpha = -\frac{1}{2} \\
x = -2t\zeta+t^{2} \rightarrow t(-2\zeta+t)
\end{cases} \\ \\ 
\end{gather}
$$
Newtonian potential for a point $(x_{0},y_{0},z_{0})$, it's brought to point, 
$$
\begin{gather}
(x,y,z) \rightarrow \frac{1}{(x-x_{0})^{2}+(y-y_{0})^{2}+(z-z_{0})^{2}}
\end{gather}
$$
is harmonic as a function on $\mathbb{R}^{3}$. To prove a function like this is harmonic, it's useful to use spherical coordinates, 
$$
\begin{gather}
\triangle = \frac{1}{r^{2}}\left( \frac{ \partial  }{ \partial r } r^{2} \frac{ \partial  }{ \partial r }  \right)
\end{gather}
$$
For an analog of $\mathbb{R}^n$, let's first think about $\mathbb{R}^{2}$, 
$$
\begin{gather}
\triangle _{\mathbb{R}^{2}} = \frac{1}{r} \left( \frac{ \partial  }{ \partial r } \frac{1}{r}\frac{ \partial  }{ \partial r }  \right)
\end{gather}
$$
we know for $n=3$, we have $r^{-1}$, for $n\geq 4$ we have $r^{2-n}$. Let's take the special case where we have a point on the $z$ axis or, 
$$
\begin{gather}
x_{0}=y_{0}=0
\end{gather}
$$
in spherical coordinates we can express the difference between the two vectors, 
$$
\begin{gather}
\frac{1}{(r_{0}^{2}-2rr_{0}\cos\theta+r^{2})^{1/2}} = \frac{1}{r_{0}} \frac{1}{\left( 1-\frac{2r}{r_{0}}\cos\theta +\left( \frac{r}{r_{0}} \right)^{2}\right)} \\ \\ 
= \frac{1}{r_{0}}\sum_{n=1}^\infty P_{n}(\cos\theta)\left( \frac{r}{r_{0}} \right)^n
\end{gather}
$$
Each term on the r.h.s is harmonic. $P_{n}$ satisfies the Legendre DE. We see the equation a little bit differently this time in terms of $\zeta$, 
$$
\begin{gather}
\left[ \frac{d}{d\zeta}\left( (1-\zeta^{2}) \frac{d}{d\zeta} \right)+n(n+1) \right]P_{n}(\zeta) = 0 \hspace{.5cm}(2)
\end{gather}
$$
As an analog of generating function for Bessel's functions, we will do a similar thing here. We'll take the $\log$ of the left hand side of function 1. we apply $t\frac{ \partial  }{ \partial t }\log$ and get,
$$
\begin{gather}
\frac{t(\zeta-t)}{(1-2t\zeta + t^{2})} = \frac{\left( \sum_{n=1}^\infty nP_{n}(\zeta)t^n \right)}{\sum_{n=0}^\infty P_{n}(\zeta)t^n} \\ \\
t(\zeta-t)\cdot \sum_{n=0}^\infty P_{n}(\zeta)t^n = (1-2t\zeta_{t^{2}}) \sum_{n=1}^\infty nP_{n}(\zeta)t^n \\ \\ 
\end{gather}
$$
Now we equate the coefficients of $t^{n+1}$, 
$$
\begin{gather}
-P_{n-1} + \zeta P_{n}(\zeta) = (n+1)P_{n+1}(\zeta) - \frac{2n\zeta P_{n}(\zeta)}{(n-1)P_{n-1}(\zeta)} \\ \\ 
\rightarrow nP_{n-1}(\zeta) - (2n+1)\zeta P_{n}(\zeta) +(n+1)P+n(\zeta)=0 
\end{gather}
$$
Now we apply, 
$$
\begin{gather}
\zeta \frac{ \partial  }{ \partial \zeta } \log \rightarrow \frac{d}{d\zeta}(P_{n+1}-P_{n-1}) =(2n+1)P_{n} 
\end{gather}
$$
Next we talk about Orthogonality of Legendre functions. We show that 
$$
\begin{gather}
\int _{0}^1 P_{n}(\zeta)P_{l}(\zeta) \, d\zeta  = 0 \hspace{.5cm} \text{if} \hspace{.2cm} n\neq l
\end{gather}
$$
furthermore, 
$$
\begin{gather}
P_{l}\frac{d}{d\zeta}\left[ (1-\zeta)^{2} \frac{dP_{n}}{d\zeta} \right]+n(n+1)P_{n}= 0 \\ \\  
P_{n}\frac{d}{d\zeta}\left[ (1-\zeta)^{2} \frac{dP_{n}}{d\zeta} \right]+l(l+1)P_{l} = 0 \\ \\ 
\frac{d}{d\zeta}(1-\zeta^{2})\left[ P_{l}  \frac{dP_{n}}{d\zeta}-P_{n} \frac{dP_{l}}{d\zeta} \right]+[n(n+1)-l(l+1)]P_{n}P_{l} = 0 \\ \\ 
\int _{-1}^1 P_{n}(\zeta)P_{l}(\zeta) \, d\zeta = 0 \hspace{.5cm} \text{ if} \hspace{.2cm} n\neq 1 \hspace{.5cm} n,l\geq 0
\end{gather}
$$
Looking back a equation 1, we can plug $1=\zeta$ to get,
$$
\begin{gather}
\frac{1}{1-t} = \sum_{n=0}^\infty \underbrace{ P_{n}(1) }_{ =1 }t^n \hspace{.5cm} \frac{1}{1+2}= \sum_{n=0}^\infty \underbrace{ P_{n}(-1 }_{ (-1)^n })t^n
\end{gather}
$$
Conclusion: $P_{0},P_{1},\dots P_{N}$ are obtained from $1,x\dots x^N$ and the gram Schmidt process normalized by $P_{1}(1)=1$. On the other hand , we'll say, 
$$
\begin{gather}
f_{n}(x) = \left( \frac{d}{dx} \right)^n (x^{2}-1)^n
\end{gather}
$$
are orthogonal to each other w.r.t 
$$
\begin{gather}
\int _{-1}^1  \, dx 
\end{gather}
$$
(an exercise is to use integration by parts to show this). We can evaluate $f_{n}(1)$,

$$
\begin{gather}
f_{n}(x) = \left( \frac{d}{dt} \right)^n [\underbrace{ (1+t)^{2}-1 }_{ (2+t)t }]^n|_{t=0} \\ \\ 
\left( \frac{d}{dt} \right)^n \underbrace{ t^n (2+t)^n }_{ 2^n t^n }+ (\text{higher order terms}) = 2^nn!
\end{gather}
$$
we can rewrite $P_{n}(x)$, 
$$
\begin{gather}
P_{n}(x) =\frac{1}{2^nn!}\left( \frac{d}{dx} \right)(x^{2}-1)^n
\end{gather}
$$
remember the beta function
$$
\begin{gather}
B(x,y) = \int _{0}^1 t^{x-1}(1-t)^{y-1} \, dx = \frac{\Gamma(x)\Gamma(y)}{\Gamma(x+y)} \\ \\
\Gamma(n+1) = n! \hspace{.5cm} \forall n \in \mathbb{N}
\end{gather}
$$
