Diffusion/Heat Equation

review improper and convergent integrals 

$$
\begin{gather}
\left( \frac{ \partial  }{ \partial t }  - \frac{ \partial^{2} }{ \partial x^{2} } \right) u(x,t) = 0 \hspace{.5cm} \text{ where k is positive and} \hspace{.2cm} t\geq 0, x \in \mathbb{R}\\ \\ 
\text{initial conditions }: u(x,0) = \phi(x) \\ \\ 
\text{1. whole line} \\ \\ 
\text{2. half line} \hspace{.2cm} x \geq 0 \hspace{.5cm} \text{boundary conditions:} \hspace{.2cm}: 
u(0,t) = \phi(t)  \\ \\ 
\text{3. closed interval}: \hspace{.2cm} a\leq x\leq b \hspace{.2cm} \text{ boundary conditions} \hspace{.2cm} u(a,t), u(b,t) 
\end{gather}
$$

This equation is a **parabolic** because the partial is second order. The highest order tells you what type of partial it.

For the wave equation, it only depends on the endpoints:
![[Pasted image 20240131121421.png|center]]


##### Whole line

We'll assume the function is given by $\phi(x)$
$$
\begin{gather}
u(x,0) = \phi(x) \hspace{.5cm} -\infty<x<\infty \\ \\ 

u(x,t) = \frac{1}{\sqrt{ 4kt }} \int_{-\infty}^{\infty} e^{-(x-y)^{2}/4kt} \psi(y) \, dy \\ \\ 
(\frac{1}{\sqrt{ 4\pi kt }})e^{-(y-x)^{2}/4kt} \hspace{.2cm} \text{as a fucntion of t} \\ \\ 

\end{gather}
$$
is the density function (for the y variable) where the mean = x and the standard deviation = $\sqrt{ 2kt }$. We take a further look at this by investigating the following equation
$$
\begin{gather}
\frac{1}{\sqrt{ 2\pi }\sigma}(e^{x^{2}/2\sigma^{2}})
\end{gather}
$$
Above is the density function of a probability distribution and is similar to the function right before this one

$$
\begin{gather}
1. \hspace{.5cm}\frac{1}{\sqrt{ 2\pi }\sigma}\int_{-\infty}^{\infty} (e^{x^{2}/2\sigma^{2}}) = 1 \, dx \\ \\ 
2. \hspace{.2cm} \int_{-\infty}^{\infty} x e^{-x^{2}/2\sigma^{2}} \, dx  =0 \\ \\ 
3. \hspace{.5cm} \frac{1}{\sqrt{ 2\pi }\sigma} \int_{-\infty}^{\infty} x^{2} e^{-x^{2}/2\sigma^{2}}\, dx = \sigma^{2}
\end{gather}
$$
1) a decaying function (improper integral) really fast from -inf to inf. We compute the integral. We can multiply the integral by itself but with x changed to y in the numerator of the power of e, and then convert to polar coordinates 

3) You can use the same method for part one

We come back to the whole line integral 
$$
\begin{gather}
u(x,t) = \frac{1}{\sqrt{ 4\pi kt }} \int_{-\infty}^{\infty} e^{-(x-y)^{2}/4kt} \psi(y) \, dy \\ \\ 

\uparrow \hspace{.2cm} \text{a continous superposition/sum of }\hspace{.2cm} \frac{1}{\sqrt{ 2kt }} e^{-(x-y)/4kt}  \\ \\ 

\left( \frac{ \partial  }{ \partial t }  - k\frac{ \partial^{2} }{ \partial x^{2} }  \right) \left( \frac{1}{\sqrt{ 4\pi kt }} \cdot e^{-(x-y)/4kt}  \right) = 0 \\ \\ 

\text{ suppose you know} \left( \frac{ \partial  }{ \partial t } - \frac{ \partial^{2} }{ \partial x^{2} }  \right) \int \left(  \frac{1}{\sqrt{ 4\pi kt }} \right) e^{-(x-y)/4kt} \psi(y)\, dy \\ \\ 

\psi(y) = \int_{-\infty}^{\infty} \left ( \frac{ \partial  }{ \partial t }  - k\frac{ \partial^{2} }{ \partial x^{2} }  \right)e^{-(x-y)/4kt} \  \, dx = 0 \\ \\ 
\end{gather}
$$
The question is at $$
\lim_{ t \to 0 } \int \left(  \frac{1}{\sqrt{ 4\pi kt }} \right) e^{-(x-y)/4kt} \psi(y)\, dy  = \psi(x) \hspace{.2cm} \text{for all} \hspace{.2cm} x\in \mathbb{R}
$$
 For $$
\lvert x-y\rvert \geq \delta \hspace{.5cm}e^{-\frac{(x-y)^{2}}{4kt}}\leq e^{-\frac{(\delta)^{2}}{4kt}}
$$
when y is close to x, in the exponent, you'll get an appretiable constant. We reword: 
$$
\begin{gather}
\lim_{ x \to 0 } \int_{-\infty}^{\infty} \frac{1}{\sqrt{ 4\pi kt }} e^{-\frac{(x-y)^{2}}{4kt}} [\psi(y)-\psi(x))]\, dy \leq \int _{x-\delta}^{x+\delta} \frac{1}{\sqrt{ 4\pi kt }} e^{-\frac{(x-y)^{2}}{4kt}} [\psi(y)-\psi(x))]\,\, dx \\ \\ 
+ \int _{\lvert x-y \rvert\geq\delta}\frac{1}{\sqrt{ 4\pi kt }} e^{-\frac{(x-y)^{2}}{4kt}} \lvert\psi(y)-\psi(x) \rvert\, \, dy \\ \\ 
\forall\epsilon >0 \hspace{.2cm} \text{choose } \hspace{.2cm} \delta \leq 1 \\ \\ 
\lvert\psi(y)-\psi(x) \rvert < \epsilon \\ \\ 

\forall y \in [x-\delta, x+\delta] \\ \\ 

\epsilon \int_{-\infty}^{\infty} {1}{\sqrt{ 4\pi kt }} e^{-\frac{(x-y)^{2}}{4kt}} 2M  \, dy \\ \\ 

\int_{\lvert x-y\rvert \geq \delta} {1}{\sqrt{ 4\pi kt }} e^{-\frac{(x-y)^{2}}{4kt}} 2M \ dy
\end{gather}
$$

We assume that:
$$
\begin{gather}
\lvert \psi(x) \rvert \leq M \hspace{.5cm} \forall x \in \mathbb{R}
\end{gather}
$$
Such that
$$
\begin{gather}
\int_{\lvert x-y\rvert \geq \delta} {1}{\sqrt{ 4\pi kt }} e^{-\frac{(x-y)^{2}}{4kt}} = \frac{1}{\sqrt{ 4\pi kt }} \int_{\lvert u\rvert \geq \delta} {1}{\sqrt{ 4\pi kt }} e^{-\frac{(u)^{2}}{4kt}} \ dy \ dy \\ \\
\text{we say:} \hspace{.2cm} z = \frac{u}{\sqrt{ 4kt }} \hspace{.5cm}dz = \frac{1}{\sqrt{ 4kt }}du \\ \\ 
\int _{\lvert z \rvert \geq \frac{\delta}{\sqrt{ 4kt }}} e^{-z^{2}}\, dz = \frac{2}{\sqrt{ \pi }}\int _{\lvert z \rvert \geq \frac{\delta}{\sqrt{ 4kt }}} e^{-z^{2}} \ dz
\end{gather}
$$
as $t \rightarrow 0$ 

Thus the integral produces a bell curve/bump function
![[Pasted image 20240131131032.png|center]]

##### Uniqueness:

Similiar to the wave equation, we use the energy method. Suppose that $u(x,0) = 0 and $\left( \frac{ \partial  }{ \partial t } - k \frac{ \partial^{2} }{ \partial x^{2} }  \right) u(x,t) = 0$

$$
\begin{gather}
E(t) = \int _{\infty}^\infty  u(x,)\, dx  \\ \\ 

\frac{d}{dt} E(t) = \int_{-\infty}^{\infty} 2u \frac{ \partial u }{ \partial x }  \, dx = \int_{-\infty}^{\infty} 2u(x,t) \cdot u_{x}(x,t) \, dx 
\end{gather}
$$
and $u(x,t)$ decays infinity and $u_{x}(x,t)$
thus the previous math line equals 
 $$
\begin{gather}
2k\int_{-\infty}^{\infty} u(x,t) \cdot U_{x x}(x,t)U \, dx \hspace{.5cm} \text{we use integration by parts} \\ \\ 

= 2k(u(x,t)u_{x}(x,t) |_{x=-\infty}^{x=\infty}) - \int_{-\infty}^{\infty} u_{x}(x,t)^{2} \, dx = -2k \int_{-\infty}^{\infty} u_{x}(x,t)^{2} \, dx \leq 0 \\ \\ 

E(0) = 0
\frac{d}{dt}E(t) \leq 0  \rightarrow E(t) = 0 \hspace{.5cm} \forall_{t} = 0 \rightarrow u(x,t) \equiv 0
\end{gather}
$$
We can also use the maximum principle to prove uniqueness

last thing:
$$
\begin{gather}
\int_{0}^{\infty} e^{-t^{2}} \, dt = \frac{\sqrt{ \pi }}{2} \\ \\

lv(f(x)) = \frac{2}{\sqrt{ \pi }}\int_{x}^{\infty} e^{-t^{2}} \, dt \\ \\ 

\frac{2}{\sqrt{ \pi }} \int_{x}^{\infty}  e^{-t^{2}}\, dt 
\end{gather}
$$
to integrate the last math line, we could use integration by parts as: 
$$
\begin{gather}
\frac{2}{\sqrt{ \pi }} \int_{x}^{\infty}  e^{-t^{2}}\, dt 
\end{gather}
$$