#### Heat equation 

$$
\begin{gather}
\frac{ \partial  }{ \partial t } = k \frac{ \partial^{2} }{ \partial x^{2} } u(x,t)= 0 \\ \\ 

-\infty < x< \infty  \hspace{.5cm} t \geq 0 \hspace{.5cm}k >0 \\ \\

\text{initial conditions} \hspace{.5cm} u(x,0) = \psi(x) \\ \\ 

u(x,t) = \frac{1}{\sqrt{ 4\pi kt }} \int_{-\infty}^{\infty} e^{-(x-y)^{2}/4kt} \psi(y)\, dy 
\end{gather}
$$
We say let  $f,g$ be the two functions on $\mathbb{R}$, then ($f*g(x)$ ) is the convolution of $f \hspace{.2cm}\text{and} \hspace{.2cm} g$ where
$$
\begin{gather}
(f*g)(x) = \int_{-\infty}^{\infty} f(x-y)g(y) \, dy  \\ \\ 
\end{gather}
$$
We mention this generally as the previous math lines helps us understand the one before it. 

$$
\begin{gather}
U(x,t) = \frac{1}{\sqrt{ 4kt }}e^{x^{2}/4kt}* \psi
\end{gather}
$$
That is the heat curve solution. 
$$
\begin{gather}
\int_{-\infty}^{\infty} e^{-t^{2}} \, dt  = \sqrt{ \pi }
\end{gather}
$$
because it's symmetric  we have that 
$$
\begin{gather}
\frac{2}{\sqrt{ \pi }}\int_{-\infty}^{\infty} e^{ -t^{2} } \, dt = 1 \\ \\ 

\psi(y)dy \hspace{.5cm}\text{Def} \hspace{.2cm} Erf_{9}x) = \frac{2}{\sqrt{ \pi }} \int _{0}^x e^{ -t^{2} }\, dt 
\end{gather}
$$
this is the error function where $x\geq 0$ keeping in mind that $\lim_{ x \to \infty }ErF(x)=1$. 

Our actual question is: what is the behavior of $1-Erf(x)$ as $x\rightarrow \infty$. Where $1-Erf(x)$ is called the complementary error function. 

Now suppose we know that $\lim_{ t \to 0 }Erfc\left( \frac{1}{t} \right) = 0$. The question rephrased, is can we find the Taylor expansion of $Erfc\left( \frac{1}{t} \right)$? Well $\forall_{n}\geq 1$, $\lim_{ t \to 0 }Erfc\left( \frac{1}{t} \right) = a_{1}t+\dots a_{n}t^n+R_{n}(t)$ and $\lvert R_{n}(t) \rvert =C_{n}t^{n+1} \hspace{.5cm} \forall_{0} < t\leq 1$. This is true $\exists C_{n} >0$.

This will be important to the problem set!

We want $\forall_{n}\geq 1$ for $\forall a_{i} \in \mathbb{R}$
$$
\begin{gather}
\int _{x}^\infty e^{ -t^{2} } \, dy = a_{1} \frac{1}{x} +a_{2} \frac{1}{x^{2}} + \dots a_{n} \frac{1}{x^n} + R_{n}(x) \hspace{.5cm} \text{and}\hspace{.5cm} \exists C_{n} > 0 \hspace{.5cm} \text{such that }\\ \\ 
\lvert R_{n}(x) \rvert \leq C_{n} \frac{1}{x^{n+1}} \hspace{.2cm} \forall_{x} \geq 100 \\ \\ 

\text{and} \hspace{.2cm} \int _{x}^\infty e^{ -t^{2} } \, dt  = \sum_{i=1}^\infty a_{i}x^{-i} \\ \\ 
\end{gather}
$$
We note to be careful when $C_{n}$ grows to fast. 

In fact we know that 
$$
\begin{gather}
\sum_{i=1}^\infty a_{i} \frac{1}{x^{i}} \hspace{.5cm} \forall_{x}>0
\end{gather}
$$
Which we know to be divergence!

$$
\begin{gather}
\sum_{i=1}^\infty a_{i} \frac{1}{x^{i}} \hspace{.5cm} \hspace{.5cm} 
\end{gather}
$$
is an asymptotic expansion of 
$$
\begin{gather}
\int _{x}^\infty e^{ -t^{2} }\, dt \hspace{.2cm} \text{at} \hspace{.2cm} x=\infty 
\end{gather}
$$

Asymptotic is an infinite divergent series. But how do we further understand the previous math line? To get to the First order approximation of that integral, we want to estimate it in terms of $x$. 
$$
\begin{gather}
\sum \frac{(-1)^n t^{2n}}{n!} = 1 - t^{2} + \frac{t^4}{2}
\end{gather}
$$
None of the terms are integrable! Let's try using integration by parts!
$$
\begin{gather}
\frac{1}{2t}e^{ -t^{2} } \cdot 2t dt = -\frac{1}{2t}e^{ -t^{2} }|_{x}^\infty - \int _{x}^\infty \frac{e^{ -t^{2} }}{2t^{2}} \, dt \\ \\ 

\text{where we have} \hspace{.2cm}-\frac{1}{2t}e^{ -t^{2} }|_{x}^\infty = \frac{e^{ -x }}{2x}
\end{gather} 
$$
now we want to investigate the second part $- \int _{x}^\infty \frac{e^{ -t^{2} }}{2t^{2}} \, dt$. We want to find a function of x that caps the inside of the integral
$$
\begin{gather}
\int _{x}^\infty \frac{e^{ -t^{2} }}{2t^{2}} \, dt  \leq \frac{1}{2x^{2}} \int _{x}^\infty e^{ -t^{2} } \, dt \leq \frac{1}{2x^{2}}\int _{0}^\infty e^{ -t^{2} }\, dt \\ \\ 

= \frac{\sqrt{ \pi }}{x^{2}}
\end{gather}
$$
$$
\begin{gather}
\int _{x}^\infty e^{ -t^{2} } \, dx \hspace{.2cm} \text{ is porportional}\\ \\ 

\frac{1}{2x} - \frac{1}{2^{2}\cdot x^{3}} + \frac{1}{2^{3} x^5} -\frac{1\cdot_{3}\cdot_{5}}{2^4}\cdot x^7 \\ \\ 

= \sum_{i=1}^\infty\frac{((-1)^{i-1} 1\cdot_{3} \dots(2i-3))}{2^{i}x^{2i-1}}
\end{gather}
$$
Thus the convention is product indexed by empty set $\phi$ is 1. Now lets look closer at the sum; 
$$
\begin{gather}
\sum_{i=1}^\infty\frac{((-1)^{i-1} 1\cdot_{3} \dots(2i-3))}{2^{i}x^{2i-1}}
\end{gather}
$$
For which x does the sum converge? How do you know if it converges for a given x? We do the ratio test!
$$
\begin{gather}
\sum_{i=1}^\infty\underbrace{ \frac{((-1)^{i-1} 1\cdot_{3} \dots(2i-3))}{2^{i}x^{2i-1}}}_{ b^i } \\ \\ 

\frac{b^{i+1}}{b^i} = (-1)\cdot \frac{2i-1}{2\cdot x^{2}}
\end{gather}
$$
the problem is that the last math line is $\geq 2$ for all $i \geq 2x^{2}$. So if $i$ is large enough the successive ratio increases 2 fold. The consequence is that this infinite series diverges $\forall x>0$



#### Heat/diffusion equation

The heat/diffusion satisfies the maximum principles (an $L^\infty$ estimate).

$$
\begin{gather}
\left( \frac{ \partial  }{ \partial t } - k\frac{ \partial^{2} }{ \partial x^{2} }  \right)(u(x,t)) = 0 \\ \\ 

a\leq x\leq b \hspace{.5cm} 0 \leq t\leq T
\end{gather}
$$
![[Pasted image 20240205130631.png|center|300]]

where $u(x,t)$ is smooth. 
$$
\begin{gather}
\text{max} \hspace{.2cm} u(x,t)=M_{a,b,T,k} \hspace{.5cm} a\leq x\leq b, \hspace{.5cm} 0\leq t\leq T \\ \\ 


\end{gather}
$$
![[Pasted image 20240205130834.png|center|300]]


Proof: 

$\forall \epsilon >0$, let $v_{\epsilon}(x,t) = u(x,t)+ \epsilon x^{2}$. Max $u(x,t)$. Suppose $u(x_{0},t_{0}) = M$. What can we say about this? 

There are two situations. One: Suppose that $0<t<M$. We can say 
$$
\begin{gather}
\frac{ \partial u}{ \partial t } (x_{0},t_{0}) = 0 \\ \\

\frac{ \partial u }{ \partial x } (x_{0},t_{0}) = 0 \\ \\ 

\frac{ \partial^{2}u }{ \partial x^{2} } (x_{0},t_{0}) \\ \\ 
\end{gather}
$$
We can say the the last math line is smooth and $\leq 0$. Max $v_{\epsilon}(x,t)= v_{\epsilon}(x_{1},t_{1})$. Thus 

$$
\begin{gather}
\frac{ \partial v_{\epsilon} }{ \partial t } (x_{1},t_{1}) = 0 \hspace{.5cm} \text{if} \hspace{.2cm} t_{1} \neq T \\ \\ 

v_{\epsilon} = u + \epsilon x  \\ \\ 

\frac{ \partial v_{\epsilon} }{ \partial t } = \frac{ \partial u }{ \partial t } = \frac{ \partial ^{2}u }{ \partial x^{2} }  = \frac{ \partial^{2} v_{\epsilon} }{ \partial x^{2} } - 2\epsilon
\end{gather}
$$