#### Maximum Principle

For the heat equation:
$$
\begin{gather}
\frac{ \partial  }{ \partial t } - k \frac{ \partial^{2} }{ \partial x^{2} } u(x,t) = 0 \\ \\

\text{where } \hspace{.2cm} u(x,t) \hspace{.2cm} \text{ is a smooth function} \hspace{.2cm} \\ \\ 

\end{gather}
$$
Consider $u(x,t)$ restricted to $a\leq x\leq b$ and $0\leq t\leq T$. Let $M = sup, (x,t) \in \hspace{.2cm} \text{in the boundary} \hspace{.2cm}$. The maximum principle: 
$$
\begin{gather}
u(x,t) \ll M \\ \\
\forall(x,t) \in [a,b] \times [0,M]
\end{gather}
$$
![[Pasted image 20240207120740.png|center|]]

Recall: We will show that $\forall_{\epsilon} >0, v_{\epsilon}(x,t) \hspace{.2cm} \text{def} \hspace{.2cm} u(x,t)+ \epsilon x^{2}\ll M+ \epsilon(b^{2}+a^{2}) = (*_{\epsilon}$. If this is true we note, if $*_{\epsilon}$ holds $\forall)\epsilon >0$, then on gets  $\forall(x,t) \in [a,b) \times[0,M]$$u(x,t) = \lim_{ \epsilon \to o+ }v_{\epsilon}(x,t) \ll M + \ll \lim_{ \epsilon \to 0 + }\epsilon x^{2}$. 

Proof: 

Given $\epsilon>0$ and that $v_{\epsilon}$ is continous, then 
$$
\begin{gather}
\exists(x_{1},t_{1}) \in [a,b]\times[0,T] \\ \\ 
\text{st} \hspace{.2cm} v_{\epsilon}(x_{1},t_{1}) = \text{sup} \hspace{.2cm} v_{\epsilon}(x,t)  \\ \\ 
\text{wher} \hspace{.2cm} (x,t)  \in [a,b]\times[0,T] \\ \\
\end{gather}
$$
Now we'll consider two cases: 
$$
\begin{gather}
if \hspace{.2cm} (x_{1}.t_{1}) \in \hspace{.2cm} \text{boundary } \hspace{.2cm} \\ \\ 

\text{then} \hspace{.2cm} v_{\epsilon}(x_{1},t_{1}) \leq M + \epsilon(b^{2}+a^{2}) \\ \\ 

v_{\epsilon}(x_{1},t_{1}) = u(x_{1},t_{1}) + \epsilon x^{2}_{1} \leq M + \epsilon(b^{2}+a^{2}) \\ \\

\end{gather}
$$
Now lets consider when $(x_{1},t_{1}) \in \epsilon(a,b) \times(0,T)$. 
$$
\begin{gather}
\left( \frac{ \partial  }{ \partial t } - \frac{ \partial^{2} }{ \partial x^{2} }  \right) v_{\epsilon}(x,t)= -2\epsilon \hspace{.5cm} \sigma
\end{gather}
$$
Now we evaluate $\sigma$ at $(x_{1},t_{1})$: $\left( \frac{ \partial  }{ \partial t } v_{\epsilon}\right(x_{1},t_{1})) = 0$. Now, 
$$
\begin{gather}
(\frac{ \partial^{2} }{ \partial x^{2}} v_{\epsilon})(x_{1},t_{1}) \leq 0
\end{gather}
$$
The consequence is that 
$$
\begin{gather}
( \frac{ \partial  }{ \partial t } - \frac{ \partial^{2} }{ \partial x^{2} }) (x_{1},t_{1})\geq 0
\end{gather}
$$
which is a contradiction as the left side we already said equals $-2\epsilon$. Now we'll suppose $t_{1}= T$. 
$$
\begin{gather}
\left( \frac{ \partial  }{ \partial t } v_{\epsilon} \right)(x_{1},T) \geq 0
\end{gather}
$$
this is true because
$$
\begin{gather}
\lim_{ h \to 0 + } \frac{v_{\epsilon}(x_{1},T) - v_{\epsilon}(x_{1},T_-h)}{h}
\end{gather}
$$
Our initial conditions :
$$
\begin{gather}
u(x,0) = \phi(x) \hspace{.5cm}x \in [a,b] \\ \\ 
u(a,t) = \psi_{1}(t) \hspace{.5cm} u(b,t) = \psi_{2}(t) \\ \\ 
\end{gather}
$$
Then this PDE with initial and boundary conditions is well posed! 

#### Wave equation
Does the maximum principle hold for the wave equation when $[a,b]\times[o,T]$? 

suppose $u(x,t)$ satisfies
$$
\begin{gather}
(\frac{ \partial^{2} }{ \partial t^{2} } )u(x,t) = 0 \\ \\ 
a\leq x\leq b \hspace{.5cm} 0 \leq t \leq T \\ \\ 
\end{gather}
$$Is it true that 
$$
\begin{gather}
u(x,t) = sup u(x,t) \hspace{.5cm} (x,t) \in \text{boundary}([a,b]\times[0,T]) \\ \\ 
\end{gather}
$$
In general, the solution would be
$$
\begin{gather}
f(x+t) + g(x-t)
\end{gather}
$$
The easiest counter example to the second to the last math line 
$$
\begin{gather}
\sin x +\sin t \hspace{.5cm} [0,\pi]\times[0,\pi] \\ \\ 

\end{gather}
$$
So now the question is the heat equation **well-posed** for negative time? We defined well-posed to be changing the coordinates and the solution properly reflects that change 
$$
\begin{gather}
\left( \frac{ \partial  }{ \partial t } - k \frac{ \partial^{2} }{ \partial x^{2} }  \right)u(x,t) = 0 \hspace{.5cm} -\infty \leq x\leq \infty \hspace{.4cm}t\leq 0\\ \\ 
\end{gather}
$$
The heat kernel is at least a working solution
$$
\begin{gather}
\int_{-\infty}^{\infty} \frac{e^{-(x-y)^{2}/4\pi kt}}{\sqrt{ 4\pi kt }} \psi \, dy
\end{gather}
$$
which we supposed $\psi(y)dy$ is concentrated near a where $\left( \frac{ \partial  }{ \partial t } - k \frac{ \partial^{2} }{ \partial x^{2} }  \right)\frac{e^{-(x-y)^{2}/4\pi kt}}{\sqrt{ 4\pi kt }} = 0 \hspace{.5cm} \forall a$ . Now we know lots of solutions, bust let's simplify the previous math line

$$
\begin{gather}
\left( \frac{ \partial  }{ \partial t } - k \frac{ \partial^{2} }{ \partial x^{2} }  \right)\int_{-\infty}^{\infty} \frac{e^{-(x-y)^{2}/4\pi kt}}{\sqrt{ 4\pi kt }} \psi \, dy
\end{gather}
$$
For $t=t_{1} < 0$ , consider $\frac{e^{-(x-y)^{2}/4\pi k(t+1)}}{\sqrt{ 4\pi kt }}$ on $-\infty<x<\infty$ and $t<0$. 
For $t=0$
$$
\begin{gather}
t=0 \hspace{.5cm} \frac{e^{-(x)^{2}/4\pi }}{\sqrt{ 4\pi k }} \\ \\

t\rightarrow \hspace{.5cm} -1^t
\end{gather} 
$$
Try to find a solution to 
$$
\begin{gather}
\left( \frac{ \partial  }{ \partial t } - \frac{ \partial^{2} }{ \partial x^{2} } u(x,t)  \right) = 0 \\ \\
\end{gather}
$$
of the form $u(x,t) = f(x) \cdot g(t)$. Well we have that
$$
\begin{gather}
f(x) \cdot g'(t) = f''(x) g(t) \\ \\ 
\frac{f''(x)}{f(x)} = \frac{g'(t)}{g(t)} = c, \hspace{.2cm} \text{a constant} \hspace{.2cm}
\end{gather}
$$
Thus we have that 
$$
\begin{gather}
g(t) = ae^{ct} \hspace{.5cm} a: \text{a constant} \hspace{.2cm} \\ \\

f(x) = \sin(-\sqrt{ c }x) + d\cos(-\sqrt{ c }x) \hspace{.5cm}c<0 \\ \\ 
\text{e.g} \hspace{.5cm}  e^{-A^{2}t}\sin(Ax) \hspace{.5cm} \text{ a solution} \hspace{.2cm} \forall a
\end{gather}
$$
Example: 
$$
\begin{gather}
e^{ -t }\sin x \hspace{.2cm} t\leq 0, \hspace{.2cm} x \in(0,\infty)
\end{gather}
$$

#### Wave Speed

 