This is what we've assumed: $u_{\sim}(x,t) = -u_{\sim}(2a-x)= -u_{\sim}(2b-x) \hspace{.2cm} \forall x \in \mathbb{R}$

#### Uniqueness
Uniqueness of a solution of 1 dim wave equation with given initial conditions. We did this with two different methods. 

Suppose we have $u_{tt} - c^{2}u_{x x} = 0$ and
$$
\begin{gather}
u(x,0) = \phi(x) \\ \\ 
\frac{ \partial u }{ \partial t } u(x,0) = \psi(x) \\ \\ 
\end{gather}
$$
We arrived here because
$$
\begin{gather}
u_{tt} - c^{2}u_{x x} = \left( \frac{ \partial  }{ \partial t } +c\frac{ \partial  }{ \partial x }  \right)\left( \frac{ \partial  }{ \partial t } -c\frac{ \partial  }{ \partial x }  \right)
\end{gather}
$$


#### Wave and heat equation with source

Wave and heat equation with source on $\mathbb{R}$ 

Heat Equation 
$$
\begin{gather}
u_{t}- ku_{x x} = f(x,t) \\ \\ 
u(x,0) = \phi(x) \hspace{.5cm} t>0, x \in \mathbb{R}
\end{gather}
$$
we have two situations: 
$$
\begin{gather}
\frac{ \partial  }{ \partial t } -k \frac{ \partial^{2} }{ \partial x^{2} } u_{1} = 0 \\ \\ 
u_{1}(x,0) = \phi(x)
\end{gather}
$$
The second equation 

$$
\begin{gather}
\frac{ \partial  }{ \partial t } -k\frac{ \partial^{2} }{ \partial x^{2} } u_{2}(x,t) = f(x,t) \\ \\
u_{2}(x,0) = 0 \\ \\ 
\lim_{ t \to 0 } u_{2}(x,t) = u_{2}(x,0)
\end{gather}
$$
Recall that $u_{1}(x,t) .  \frac{1}{\sqrt{ 4\pi kt }} \int \text{heat kernel} \phi(y)\, dy$
$$
\begin{gather}
u_{2}(x,t) = \iint_{t>s>0} \frac{e^{ -(x-y)^{2}/4k(t-s) }}{\sqrt{ 4\pi k(t-s) }} f(y,s) \, dyds \\ \\ 
\int _{0}^t  \, ds \int _{\infty}^\infty \frac{e^{ -(x-y)^{2}/4k(t-s) }}{\sqrt{ 4\pi k(t-s) }} f(y,s) \, dy  \\ \\ 

\frac{ \partial u }{ \partial t } (x,t) = \lim_{ s \to t^- } \int _{-\infty}^\infty \frac{e^{ -(x-y)^{2}/4k(t-s) }}{\sqrt{ 4\pi k(t-s) }} f(y,s) \, dx + \\ \\
\int _{0}^t \, ds \int_{-\infty}^{\infty}\left(  \frac{ \partial  }{ \partial t } -\frac{ \partial  }{ \partial x^{2} } \right)(\frac{e^{ -(x-y)^{2}/4k(t-s) }}{\sqrt{ 4\pi k(t-s) }} f(y,s))  \, dx 
\end{gather}
$$
The last math line was achieved by the chain rule. Remember we showed; 
$$
\begin{gather}
\lim_{ \epsilon \to 0^+ } \int_{-\infty}^{\infty} \frac{e^{ -(x-y)^{2}/\sqrt{ 4k\epsilon } }}{\sqrt{ 4\pi\epsilon }} \phi(y) \, dy 
\end{gather}
$$
when $\epsilon$ is small its a very narrow bump. 