Exam information:
- 5 exam problems 
- 2 extra credit problems
  
  
  #### Wave equation 
  Wave equation with a source with space dim = 1
  $$
\begin{gather}
\left( \frac{ \partial^{2} }{ \partial t^{2} } -c\frac{ \partial^{2} }{ \partial x^{2} }  \right)u = f(x) \\ \\ 
u(x,0) = \phi(x) \\ \\ 
\frac{ \partial u }{ \partial t } (x,0) = \psi(x) \\ \\ 

\end{gather}
$$
We use this for two solutions
$$
\begin{gather}
\left( \frac{ \partial^{2} }{ \partial t^{2} } -c^{2}\frac{ \partial^{2} }{ \partial x^{2} }  \right) u_{1}=0 \\ \\ 

u_{1}(x,0) = \phi(x) \\ \\ 
\frac{ \partial u_{1} }{ \partial t } (x,0) = \psi(x) \\ \\ 
\end{gather}
$$

and 
$$
\begin{gather}
\left( \frac{ \partial^{2} }{ \partial t^{2} } -c^{2}\frac{ \partial^{2} }{ \partial x^{2} }  \right) u_{2} = f(x,t) \\ \\ 
u_{2}(x,0) = 0 \\ \\ 
\frac{ \partial u_{2} }{ \partial t } (x,0) = 0 
\end{gather}
$$
there are many ways to solve the above two equations, but let's do the easiest way: 
$$
\begin{gather}
\left( \frac{ \partial^{2} }{ \partial t^{2} } -c^{2}\frac{ \partial^{2} }{ \partial x^{2} }  \right) = \left( \frac{ \partial  }{ \partial t } +c\frac{ \partial  }{ \partial x }  \right)\left( \frac{ \partial  }{ \partial t } -c\frac{ \partial  }{ \partial x }  \right) \\ \\ 


\end{gather}
$$
we transform into the new coordinate system: 
$$
\begin{gather}
y = x-ct \\ \\ 

z = x+ct \\ \\ 

\frac{ \partial  }{ \partial t } = \frac{ \partial y }{ \partial t } \frac{ \partial  }{ \partial y } + \frac{ \partial z }{ \partial t } \frac{ \partial  }{ \partial z }  = -c \frac{ \partial  }{ \partial y } +c\frac{ \partial  }{ \partial z } \\ \\ 

\frac{ \partial  }{ \partial x } = \frac{ \partial y }{ \partial x } \frac{ \partial  }{ \partial y }  + \frac{ \partial z }{ \partial x } \frac{ \partial  }{ \partial z }  = \frac{ \partial  }{ \partial y } + \frac{ \partial  }{ \partial z }  \\ \\ 

\frac{ \partial  }{ \partial t } +c\frac{ \partial  }{ \partial x }  = 2c \frac{ \partial  }{ \partial z }  \\ \\ 

\frac{ \partial  }{ \partial t } -c\frac{ \partial  }{ \partial x }  = -2c\frac{ \partial  }{ \partial y } 
\end{gather}  
$$
how do we solve this? 

$$
\begin{gather}
\text{Let} F(y,z)= f\left( \frac{y+z}{2}, \frac{z-y}{2c} \right) \hspace{.2cm} \\ \\ 

\text{where} \hspace{.2cm} x= \frac{y+z}{2} \hspace{.5cm} t= \frac{z-y}{2c} \\ \\ 

v_{2}(y,z) = u_{2} \left( \frac{y+z}{2}, \frac{z-y}{2} \right) \\ \\ 

\begin{cases}
\frac{ \partial^{2}v }{ \partial y \partial z }  = -\frac{1}{4c^{2}}F(y,z) \\ 
v_{2}(y,y) = 0 \\ 
\end{cases} \\ \\

\frac{ \partial u_{2} }{ \partial t }  = -c\frac{ \partial v_{2} }{ \partial y } +c\frac{ \partial v_{2} }{ \partial z } \\ \\ 

\frac{ \partial 'v_{2} }{ \partial y } (y,y) = -\frac{ \partial v_{2} }{ \partial z } (y,y) \\ \\ 

\frac{ \partial^{2}v }{ \partial y\partial z } (y,z) = G(y,z) \\ \\ 

\text{where} \hspace{.2cm} \frac{ \partial^{2}v }{ \partial y\partial z } (y,z) = G(y,z) \\ \\ 

\end{gather}
$$
we continue 
$$
\begin{gather}
\frac{ \partial v }{ \partial z } (y,z_{0}) = \frac{ \partial v }{ \partial y } (y_{0},z)+\int _{y_{0}}^y G(y,z) \, dy \\ \\ 
\text{integrate once more} \hspace{.2cm} \\ \\ 

v(y,z) = \int_{z_{0}}^z \frac{ \partial v }{ \partial y } (y_{0},z) \, dx  +\frac{ \partial v }{ \partial y } (y_{0},z_{0})+\int _{z_{0}}^z \, dz \int _{y_{0}}^y G(y,z) \, dy 
\end{gather}
$$
in the book they tell us
$$
\begin{gather}
\frac{1}{2c} \iint_{\triangle}f  \, dx 
\end{gather}
$$
![[Pasted image 20240219123644.png|center]]


#### Separation of variables

The domain of the function in the PDE  and the PDE itself have suitable symmetry.

When this applies: Reduce to ODE

Example: Heat equation on finite interval 
$$
\begin{gather}
k>0  \\ \\ 
\left( \frac{ \partial  }{ \partial t } -k\frac{ \partial  }{ \partial x^{2} }  \right) u(x,t) = 0 \hspace{.5cm} 0\leq x\leq L \hspace{.5cm} t\geq 0\\ \\ 
\end{gather}
$$
initial condition
$$
\begin{gather}
\lim_{ t \to o+ }u(x,t) = \phi(x) \hspace{.5cm}\forall 0\leq x\leq L \\ \\ 

\begin{cases}
u(0,t) = 0  \\
u(L,t) = 0 
\end{cases} \\ \\ 
\text{homog Dirichlet boundary condition} \hspace{.2cm}
\end{gather}
$$

Main idea: 
- try to find simple solutions of the form $u(x,y) = f(x)g(t)$ for suitable functions $f(x) \hspace{.5cm} 0\leq x\leq L  \hspace{.5cm} g(t) \hspace{.5cm}0\leq t$ which satisfies the homogenous boundary conditions
- Try to find a suitable linear combination of solutions found in step 1 which satisfies the given initial condition 

$$
\begin{gather}
\left( \frac{ \partial  }{ \partial t }  - k \frac{ \partial^{2} }{ \partial x^{2} }  \right)f(x)g(t) = f(x)g'(t)- kf''(x)g(t) \hspace{.5cm}\forall x\in[0,L] \hspace{.5cm} \forall t\in[0,\infty] \\ \\ 

k\frac{f''(x)}{f(x)} =\frac{g'(t)}{g(t)} = \text{a constant, c} \hspace{.2cm} \\ \\

\frac{f''(x)}{f(x)} = \frac{c}{k} \hspace{.5cm} \frac{g'(t)}{g(t)} = c \\ \\ 

g(t) = de^{ ct } \hspace{.5cm} d\neq 0,\hspace{.2cm} \text{a constant} \hspace{.2cm} \\ \\ 

f''(x) = \frac{c}{k}f(x) \hspace{.5cm} \forall \hspace{.5cm}x\in [0,L] \\ \\ 

f(0) = f(L) = 0 \\ \\ 

\frac{c}{k}= 0 \rightarrow f(x) = 0 \\ \\ 

\frac{c}{k}>0 \rightarrow f(x) = 0 \\ \\ 

c<0 \hspace{.5cm}f(x) = A\cos\left( \frac{\sqrt{ c }}{k}x \right)+ B\sin\left( \sqrt{ -\frac{c}{k} }x \right)
\end{gather}
$$
for suitable $A,B \in \mathbb{R}$
$$
\begin{gather}
0 = f(x) = A \\ \\ 
\text{need}: \hspace{.2cm} \sin\left( \frac{\sqrt{ -c }}{k}L \right) = 0 \\ \\

\sqrt{ -\frac{c}{k} }L \in \mathbb{Z} \pi \hspace{.5cm} \exists n\in\mathbb{Z} \\ \\ 
-c = \frac{kn^{2}\pi^{2}}{L} \\ \\ 
c = - \frac{k\pi^{2}n^{2}}{L^{2}}
\end{gather}
$$
Thus we get solutions of the form 
$$
\begin{gather}
\sin\left( \frac{\pi}{L}n x\right)e^{ -\frac{k\pi n^{2}}{L^{2}} }t \hspace{.5cm} n\in \mathbb{Z}
\end{gather}
$$

Now we need to try to find suitable numbers $b_{n}$ $n\in$ such that

$$
\begin{gather}
\sum_{n=1}^\infty b_{n}\sin\left( \frac{\pi}{2}nx \right)e^{ -k\pi^{2} n^{2}t/L^{2} }
\end{gather}
$$

converges to a solution we need/want. Need: 
$$
\begin{gather}
\sum_{n=1}^\infty b_{n}\sin\left( \frac{\pi n}{L}x \right) = f(x) \hspace{.5cm} \forall x\in[0,L]
\end{gather}
$$